wip: bignum32

code/bignum/Hacl.Spec.Bignum.Addition.fst
@@ -12,18 +12,18 @@ open Hacl.Spec.Lib
 
 #reset-options "--z3rlimit 50 --fuel 0 --ifuel 0"
 
-val bn_sub1_f: #aLen:size_nat -> a:lbignum aLen -> i:size_nat{i < aLen} -> c_in:carry -> carry & uint64
-let bn_sub1_f #aLen a i c_in = subborrow_u64 c_in a.[i] (u64 0)
+val bn_sub1_f: #t:limb_t -> #aLen:size_nat -> a:lbignum t aLen -> i:size_nat{i < aLen} -> c_in:carry t -> carry t & limb t
+let bn_sub1_f #t #aLen a i c_in = subborrow c_in a.[i] (uint #t 0)
 
-val bn_sub1: #aLen:size_nat -> a:lbignum aLen -> c_in:carry -> tuple2 carry (lbignum aLen)
-let bn_sub1 #aLen a c_in = generate_elems #uint64 #carry aLen aLen (bn_sub1_f a) c_in
+val bn_sub1: #t:limb_t -> #aLen:size_nat -> a:lbignum t aLen -> c_in:carry t -> tuple2 (carry t) (lbignum t aLen)
+let bn_sub1 #t #aLen a c_in = generate_elems aLen aLen (bn_sub1_f a) c_in
 
-val bn_sub_f: #aLen:size_nat -> a:lbignum aLen -> b:lbignum aLen -> i:size_nat{i < aLen} -> c:carry -> carry & uint64
-let bn_sub_f #aLen a b i c = subborrow_u64 c a.[i] b.[i]
+val bn_sub_f: #t:limb_t -> #aLen:size_nat -> a:lbignum t aLen -> b:lbignum t aLen -> i:size_nat{i < aLen} -> c:carry t -> carry t & limb t
+let bn_sub_f #t #aLen a b i c = subborrow c a.[i] b.[i]
 
-val bn_sub: #aLen:size_nat -> #bLen:size_nat{bLen <= aLen} -> a:lbignum aLen -> b:lbignum bLen -> tuple2 carry (lbignum aLen)
-let bn_sub #aLen #bLen a b =
-  let c0, res0 = generate_elems #uint64 #carry bLen bLen (bn_sub_f (sub a 0 bLen) b) (u64 0) in
+val bn_sub: #t:limb_t -> #aLen:size_nat -> #bLen:size_nat{bLen <= aLen} -> a:lbignum t aLen -> b:lbignum t bLen -> tuple2 (carry t) (lbignum t aLen)
+let bn_sub #t #aLen #bLen a b =
+  let c0, res0 = generate_elems bLen bLen (bn_sub_f (sub a 0 bLen) b) (uint #t 0) in
 
   if bLen < aLen then
     let c1, res1 = bn_sub1 (sub a bLen (aLen - bLen)) c0 in
@@ -31,18 +31,18 @@ let bn_sub #aLen #bLen a b =
   else c0, res0
 
 
-val bn_add1_f: #aLen:size_nat -> a:lbignum aLen -> i:size_nat{i < aLen} -> c_in:carry -> carry & uint64
-let bn_add1_f #aLen a i c_in = addcarry_u64 c_in a.[i] (u64 0)
+val bn_add1_f: #t:limb_t -> #aLen:size_nat -> a:lbignum t aLen -> i:size_nat{i < aLen} -> c_in:carry t -> carry t & limb t
+let bn_add1_f #t #aLen a i c_in = addcarry c_in a.[i] (uint #t 0)
 
-val bn_add1: #aLen:size_nat -> a:lbignum aLen -> c_in:carry -> tuple2 carry (lbignum aLen)
-let bn_add1 #aLen a c_in = generate_elems #uint64 #carry aLen aLen (bn_add1_f a) c_in
+val bn_add1: #t:limb_t -> #aLen:size_nat -> a:lbignum t aLen -> c_in:carry t -> tuple2 (carry t) (lbignum t aLen)
+let bn_add1 #t #aLen a c_in = generate_elems aLen aLen (bn_add1_f a) c_in
 
-val bn_add_f: #aLen:size_nat -> a:lbignum aLen -> b:lbignum aLen -> i:size_nat{i < aLen} -> c:carry -> carry & uint64
-let bn_add_f #aLen a b i c = addcarry_u64 c a.[i] b.[i]
+val bn_add_f: #t:limb_t -> #aLen:size_nat -> a:lbignum t aLen -> b:lbignum t aLen -> i:size_nat{i < aLen} -> c:carry t -> carry t & limb t
+let bn_add_f #t #aLen a b i c = addcarry c a.[i] b.[i]
 
-val bn_add: #aLen:size_nat -> #bLen:size_nat{bLen <= aLen} -> a:lbignum aLen -> b:lbignum bLen -> carry & lbignum aLen
-let bn_add #aLen #bLen a b =
-  let c0, res0 = generate_elems #uint64 #carry bLen bLen (bn_add_f (sub a 0 bLen) b) (u64 0) in
+val bn_add: #t:limb_t -> #aLen:size_nat -> #bLen:size_nat{bLen <= aLen} -> a:lbignum t aLen -> b:lbignum t bLen -> carry t & lbignum t aLen
+let bn_add #t #aLen #bLen a b =
+  let c0, res0 = generate_elems bLen bLen (bn_add_f (sub a 0 bLen) b) (uint #t 0) in
 
   if bLen < aLen then
     let c1, res1 = bn_add1 (sub a bLen (aLen - bLen)) c0 in
@@ -51,382 +51,396 @@ let bn_add #aLen #bLen a b =
 
 
 val bn_add1_lemma_loop_step:
-    #aLen:size_nat
-  -> a:lbignum aLen
-  -> c_in:carry
+    #t:limb_t
+  -> #aLen:size_nat
+  -> a:lbignum t aLen
+  -> c_in:carry t
   -> i:pos{i <= aLen}
-  -> c1_res1:generate_elem_a uint64 carry aLen (i - 1)
-  -> Lemma
+  -> c1_res1:generate_elem_a (limb t) (carry t) aLen (i - 1) -> Lemma
   (requires
    (let (c1, res1) = c1_res1 in
-    v c1 * pow2 (64 * (i - 1)) + bn_v #(i - 1) res1 == eval_ aLen a (i - 1) + v c_in))
+    v c1 * pow2 (bits t * (i - 1)) + bn_v #t #(i - 1) res1 == eval_ aLen a (i - 1) + v c_in))
   (ensures
-   (let (c_out, res) = generate_elem_f #uint64 #carry aLen (bn_add1_f a) (i - 1) c1_res1 in
-    v c_out * pow2 (64 * i) + bn_v #i res == eval_ aLen a i + v c_in))
+   (let (c_out, res) = generate_elem_f aLen (bn_add1_f a) (i - 1) c1_res1 in
+    v c_out * pow2 (bits t * i) + bn_v #t #i res == eval_ aLen a i + v c_in))
 
-let bn_add1_lemma_loop_step #aLen a c_in i (c1, res1) =
-  let (c_out, res) = generate_elem_f #uint64 #carry aLen (bn_add1_f a) (i - 1) (c1, res1) in
+let bn_add1_lemma_loop_step #t #aLen a c_in i (c1, res1) =
+  let (c_out, res) = generate_elem_f aLen (bn_add1_f a) (i - 1) (c1, res1) in
   let c, e = bn_add1_f a (i - 1) c1 in
-  assert (v e + v c * pow2 64 == v a.[i - 1] + v c1);
+  assert (v e + v c * pow2 (bits t) == v a.[i - 1] + v c1);
+  let p = bits t in
 
   calc (==) {
-    v c * pow2 (64 * i) + bn_v #i res;
-    (==) { bn_eval_snoc #(i - 1) res1 e }
-    v c * pow2 (64 * i) + bn_v #(i - 1) res1 + v e * pow2 (64 * (i - 1));
+    v c * pow2 (p * i) + bn_v #t #i res;
+    (==) { bn_eval_snoc #t #(i - 1) res1 e }
+    v c * pow2 (p * i) + bn_v #t #(i - 1) res1 + v e * pow2 (p * (i - 1));
     (==) { }
-    v c * pow2 (64 * i) + eval_ aLen a (i - 1) + v c_in - (v e + v c * pow2 64 - v a.[i - 1]) * pow2 (64 * (i - 1)) + v e * pow2 (64 * (i - 1));
-    (==) { Math.Lemmas.distributivity_sub_left (v e) (v e + v c * pow2 64 - v a.[i - 1]) (pow2 (64 * (i - 1))) }
-    v c * pow2 (64 * i) + eval_ aLen a (i - 1) + v c_in + (v e - v e - v c * pow2 64 + v a.[i - 1]) * pow2 (64 * (i - 1));
-    (==) { Math.Lemmas.distributivity_sub_left (v a.[i - 1]) (v c * pow2 64) (pow2 (64 * (i - 1))) }
-    v c * pow2 (64 * i) + eval_ aLen a (i - 1) + v c_in + v a.[i - 1] * pow2 (64 * (i - 1)) - v c * pow2 64 * pow2 (64 * (i - 1));
-    (==) { Math.Lemmas.paren_mul_right (v c) (pow2 64) (pow2 (64 * (i - 1))); Math.Lemmas.pow2_plus 64 (64 * (i - 1)) }
-    eval_ aLen a (i - 1) + v c_in + v a.[i - 1] * pow2 (64 * (i - 1));
-    (==) { bn_eval_unfold_i #aLen a i }
+    v c * pow2 (p * i) + eval_ aLen a (i - 1) + v c_in - (v e + v c * pow2 p - v a.[i - 1]) * pow2 (p * (i - 1)) + v e * pow2 (p * (i - 1));
+    (==) { Math.Lemmas.distributivity_sub_left (v e) (v e + v c * pow2 p - v a.[i - 1]) (pow2 (p * (i - 1))) }
+    v c * pow2 (p * i) + eval_ aLen a (i - 1) + v c_in + (v e - v e - v c * pow2 p + v a.[i - 1]) * pow2 (p * (i - 1));
+    (==) { Math.Lemmas.distributivity_sub_left (v a.[i - 1]) (v c * pow2 p) (pow2 (p * (i - 1))) }
+    v c * pow2 (p * i) + eval_ aLen a (i - 1) + v c_in + v a.[i - 1] * pow2 (p * (i - 1)) - v c * pow2 p * pow2 (p * (i - 1));
+    (==) { Math.Lemmas.paren_mul_right (v c) (pow2 p) (pow2 (p * (i - 1))); Math.Lemmas.pow2_plus p (p * (i - 1)) }
+    eval_ aLen a (i - 1) + v c_in + v a.[i - 1] * pow2 (p * (i - 1));
+    (==) { bn_eval_unfold_i #t #aLen a i }
     eval_ aLen a i + v c_in;
   };
-  assert (v c * pow2 (64 * i) + bn_v #i res == eval_ aLen a i + v c_in)
+  assert (v c * pow2 (p * i) + bn_v #t #i res == eval_ aLen a i + v c_in)
 
 
 val bn_add1_lemma_loop:
-    #aLen:size_nat
-  -> a:lbignum aLen
-  -> c_in:carry
-  -> i:nat{i <= aLen} -> Lemma
-  (let (c_out, res) : generate_elem_a uint64 carry aLen i = generate_elems #uint64 #carry aLen i (bn_add1_f a) c_in in
-   v c_out * pow2 (64 * i) + bn_v #i res == eval_ aLen a i + v c_in)
+    #t:limb_t
+  -> #aLen:size_nat
+  -> a:lbignum t aLen
+  -> c_in:carry t
+  -> i:nat{i <= aLen} ->
+  Lemma (let (c_out, res) : generate_elem_a (limb t) (carry t) aLen i = generate_elems aLen i (bn_add1_f a) c_in in
+   v c_out * pow2 (bits t * i) + bn_v #t #i res == eval_ aLen a i + v c_in)
 
-let rec bn_add1_lemma_loop #aLen a c_in i =
-  let (c_out, res) : generate_elem_a uint64 carry aLen i = generate_elems #uint64 #carry aLen i (bn_add1_f a) c_in in
+let rec bn_add1_lemma_loop #t #aLen a c_in i =
+  let p = bits t in
+  let (c_out, res) : generate_elem_a (limb t) (carry t) aLen i = generate_elems aLen i (bn_add1_f a) c_in in
   if i = 0 then begin
-    eq_generate_elems0 #uint64 #carry aLen i (bn_add1_f a) c_in;
+    eq_generate_elems0 aLen i (bn_add1_f a) c_in;
     assert (c_out == c_in /\ res == Seq.empty);
-    bn_eval0 #0 res;
+    bn_eval0 #t #0 res;
     assert_norm (pow2 0 = 1);
     bn_eval0 a;
     () end
   else begin
-    let (c1, res1) : generate_elem_a uint64 carry aLen (i - 1) = generate_elems #uint64 #carry aLen (i - 1) (bn_add1_f a) c_in in
-    generate_elems_unfold #uint64 #carry aLen i (bn_add1_f a) c_in (i - 1);
-    assert (generate_elems #uint64 #carry aLen i (bn_add1_f a) c_in ==
-      generate_elem_f aLen (bn_add1_f a) (i - 1) (generate_elems #uint64 #carry aLen (i - 1) (bn_add1_f a) c_in));
-    assert ((c_out, res) == generate_elem_f #uint64 #carry aLen (bn_add1_f a) (i - 1) (c1, res1));
-    bn_add1_lemma_loop #aLen a c_in (i - 1);
-    assert (v c1 * pow2 (64 * (i - 1)) + bn_v #(i - 1) res1 == eval_ aLen a (i - 1) + v c_in);
-    bn_add1_lemma_loop_step #aLen a c_in i (c1, res1);
-    assert (v c_out * pow2 (64 * i) + bn_v #i res == eval_ aLen a i + v c_in);
+    let (c1, res1) : generate_elem_a (limb t) (carry t) aLen (i - 1) = generate_elems aLen (i - 1) (bn_add1_f a) c_in in
+    generate_elems_unfold aLen i (bn_add1_f a) c_in (i - 1);
+    assert (generate_elems aLen i (bn_add1_f a) c_in ==
+      generate_elem_f aLen (bn_add1_f a) (i - 1) (generate_elems aLen (i - 1) (bn_add1_f a) c_in));
+    assert ((c_out, res) == generate_elem_f aLen (bn_add1_f a) (i - 1) (c1, res1));
+    bn_add1_lemma_loop a c_in (i - 1);
+    assert (v c1 * pow2 (p * (i - 1)) + bn_v #t #(i - 1) res1 == eval_ aLen a (i - 1) + v c_in);
+    bn_add1_lemma_loop_step a c_in i (c1, res1);
+    assert (v c_out * pow2 (p * i) + bn_v #t #i res == eval_ aLen a i + v c_in);
     () end
 
 
-val bn_add1_lemma: #aLen:size_nat -> a:lbignum aLen -> c_in:carry ->
-  Lemma
-  (let (c_out, res) = bn_add1 #aLen a c_in in
-   v c_out * pow2 (64 * aLen) + bn_v res == bn_v a + v c_in)
+val bn_add1_lemma: #t:limb_t -> #aLen:size_nat -> a:lbignum t aLen -> c_in:carry t ->
+  Lemma (let (c_out, res) = bn_add1 a c_in in
+   v c_out * pow2 (bits t * aLen) + bn_v res == bn_v a + v c_in)
 
-let bn_add1_lemma #aLen a c_in =
-  let (c_out, res) = bn_add1 #aLen a c_in in
-  bn_add1_lemma_loop #aLen a c_in aLen
+let bn_add1_lemma #t #aLen a c_in =
+  let (c_out, res) = bn_add1 a c_in in
+  bn_add1_lemma_loop a c_in aLen
 
 
 val bn_add_lemma_loop_step:
-    #aLen:size_nat
-  -> a:lbignum aLen
-  -> b:lbignum aLen
+    #t:limb_t
+  -> #aLen:size_nat
+  -> a:lbignum t aLen
+  -> b:lbignum t aLen
   -> i:pos{i <= aLen}
-  -> c1_res1:generate_elem_a uint64 carry aLen (i - 1)
-  -> Lemma
+  -> c1_res1:generate_elem_a (limb t) (carry t) aLen (i - 1) -> Lemma
   (requires
    (let (c1, res1) = c1_res1 in
-    v c1 * pow2 (64 * (i - 1)) + bn_v #(i - 1) res1 == eval_ aLen a (i - 1) + eval_ aLen b (i - 1)))
+    v c1 * pow2 (bits t * (i - 1)) + bn_v #t #(i - 1) res1 == eval_ aLen a (i - 1) + eval_ aLen b (i - 1)))
   (ensures
    (let (c1, res1) = c1_res1 in
-    let (c, res) = generate_elem_f #uint64 #carry aLen (bn_add_f a b) (i - 1) (c1, res1) in
-    v c * pow2 (64 * i) + bn_v #i res == eval_ aLen a i + eval_ aLen b i))
+    let (c, res) = generate_elem_f aLen (bn_add_f a b) (i - 1) (c1, res1) in
+    v c * pow2 (bits t * i) + bn_v #t #i res == eval_ aLen a i + eval_ aLen b i))
 
-let bn_add_lemma_loop_step #aLen a b i (c1, res1) =
-  let (c, res) = generate_elem_f #uint64 #carry aLen (bn_add_f a b) (i - 1) (c1, res1) in
+let bn_add_lemma_loop_step #t #aLen a b i (c1, res1) =
+  let p = bits t in
+  let (c, res) = generate_elem_f aLen (bn_add_f a b) (i - 1) (c1, res1) in
   let c, e = bn_add_f a b (i - 1) c1 in
-  assert (v e + v c * pow2 64 == v a.[i - 1] + v b.[i - 1] + v c1);
+  assert (v e + v c * pow2 p == v a.[i - 1] + v b.[i - 1] + v c1);
 
   calc (==) {
-    v c * pow2 (64 * i) + bn_v #i res;
-    (==) { bn_eval_snoc #(i - 1) res1 e }
-    v c * pow2 (64 * i) + bn_v #(i - 1) res1 + v e * pow2 (64 * (i - 1));
+    v c * pow2 (p * i) + bn_v #t #i res;
+    (==) { bn_eval_snoc #t #(i - 1) res1 e }
+    v c * pow2 (p * i) + bn_v #t #(i - 1) res1 + v e * pow2 (p * (i - 1));
     (==) { }
-    v c * pow2 (64 * i) + eval_ aLen a (i - 1) + eval_ aLen b (i - 1) - (v e + v c * pow2 64 - v a.[i - 1] - v b.[i - 1]) * pow2 (64 * (i - 1)) + v e * pow2 (64 * (i - 1));
-    (==) { Math.Lemmas.distributivity_sub_left (v e) (v e + v c * pow2 64 - v a.[i - 1] - v b.[i - 1]) (pow2 (64 * (i - 1))) }
-    v c * pow2 (64 * i) + eval_ aLen a (i - 1) + eval_ aLen b (i - 1) + (v e - v e - v c * pow2 64 + v a.[i - 1] + v b.[i - 1]) * pow2 (64 * (i - 1));
-    (==) { Math.Lemmas.distributivity_sub_left (v a.[i - 1] + v b.[i - 1]) (v c1 * pow2 64) (pow2 (64 * (i - 1))) }
-    v c * pow2 (64 * i) + eval_ aLen a (i - 1) + eval_ aLen b (i - 1) + (v a.[i - 1] + v b.[i - 1]) * pow2 (64 * (i - 1)) - v c * pow2 64 * pow2 (64 * (i - 1));
-    (==) { Math.Lemmas.paren_mul_right (v c) (pow2 64) (pow2 (64 * (i - 1))); Math.Lemmas.pow2_plus 64 (64 * (i - 1)) }
-    eval_ aLen a (i - 1) + eval_ aLen b (i - 1) + (v a.[i - 1] + v b.[i - 1]) * pow2 (64 * (i - 1));
-    (==) { Math.Lemmas.distributivity_add_left (v a.[i - 1]) (v b.[i - 1]) (pow2 (64 * (i - 1))) }
-    eval_ aLen a (i - 1) + eval_ aLen b (i - 1) + v a.[i - 1] * pow2 (64 * (i - 1)) + v b.[i - 1] * pow2 (64 * (i - 1));
-    (==) { bn_eval_unfold_i #aLen a i }
-    eval_ aLen a i + eval_ aLen b (i - 1) + v b.[i - 1] * pow2 (64 * (i - 1));
-    (==) { bn_eval_unfold_i #aLen b i }
+    v c * pow2 (p * i) + eval_ aLen a (i - 1) + eval_ aLen b (i - 1) - (v e + v c * pow2 p - v a.[i - 1] - v b.[i - 1]) * pow2 (p * (i - 1)) + v e * pow2 (p * (i - 1));
+    (==) { Math.Lemmas.distributivity_sub_left (v e) (v e + v c * pow2 p - v a.[i - 1] - v b.[i - 1]) (pow2 (p * (i - 1))) }
+    v c * pow2 (p * i) + eval_ aLen a (i - 1) + eval_ aLen b (i - 1) + (v e - v e - v c * pow2 p + v a.[i - 1] + v b.[i - 1]) * pow2 (p * (i - 1));
+    (==) { Math.Lemmas.distributivity_sub_left (v a.[i - 1] + v b.[i - 1]) (v c1 * pow2 p) (pow2 (p * (i - 1))) }
+    v c * pow2 (p * i) + eval_ aLen a (i - 1) + eval_ aLen b (i - 1) + (v a.[i - 1] + v b.[i - 1]) * pow2 (p * (i - 1)) - v c * pow2 p * pow2 (p * (i - 1));
+    (==) { Math.Lemmas.paren_mul_right (v c) (pow2 p) (pow2 (p * (i - 1))); Math.Lemmas.pow2_plus p (p * (i - 1)) }
+    eval_ aLen a (i - 1) + eval_ aLen b (i - 1) + (v a.[i - 1] + v b.[i - 1]) * pow2 (p * (i - 1));
+    (==) { Math.Lemmas.distributivity_add_left (v a.[i - 1]) (v b.[i - 1]) (pow2 (p * (i - 1))) }
+    eval_ aLen a (i - 1) + eval_ aLen b (i - 1) + v a.[i - 1] * pow2 (p * (i - 1)) + v b.[i - 1] * pow2 (p * (i - 1));
+    (==) { bn_eval_unfold_i #t #aLen a i }
+    eval_ aLen a i + eval_ aLen b (i - 1) + v b.[i - 1] * pow2 (p * (i - 1));
+    (==) { bn_eval_unfold_i #t #aLen b i }
     eval_ aLen a i + eval_ aLen b i;
   };
-  assert (v c * pow2 (64 * i) + bn_v #i res == eval_ aLen a i + eval_ aLen b i)
+  assert (v c * pow2 (p * i) + bn_v #t #i res == eval_ aLen a i + eval_ aLen b i)
 
 
 val bn_add_lemma_loop:
-    #aLen:size_nat
-  -> a:lbignum aLen
-  -> b:lbignum aLen
-  -> i:nat{i <= aLen} -> Lemma
-  (let (c, res) : generate_elem_a uint64 carry aLen i = generate_elems #uint64 #carry aLen i (bn_add_f a b) (u64 0) in
-   v c * pow2 (64 * i) + bn_v #i res == eval_ aLen a i + eval_ aLen b i)
+    #t:limb_t
+  -> #aLen:size_nat
+  -> a:lbignum t aLen
+  -> b:lbignum t aLen
+  -> i:nat{i <= aLen} ->
+  Lemma (let (c, res) : generate_elem_a (limb t) (carry t) aLen i = generate_elems aLen i (bn_add_f a b) (uint #t 0) in
+   v c * pow2 (bits t * i) + bn_v #t #i res == eval_ aLen a i + eval_ aLen b i)
 
-let rec bn_add_lemma_loop #aLen a b i =
-  let (c, res) : generate_elem_a uint64 carry aLen i = generate_elems #uint64 #carry aLen i (bn_add_f a b) (u64 0) in
+let rec bn_add_lemma_loop #t #aLen a b i =
+  let p = bits t in
+  let (c, res) : generate_elem_a (limb t) (carry t) aLen i = generate_elems aLen i (bn_add_f a b) (uint #t 0) in
   if i = 0 then begin
-    eq_generate_elems0 #uint64 #carry aLen i (bn_add_f a b) (u64 0);
-    assert (c == u64 0 /\ res == Seq.empty);
-    bn_eval0 #0 res;
+    eq_generate_elems0 aLen i (bn_add_f a b) (uint #t 0);
+    assert (c == uint #t 0 /\ res == Seq.empty);
+    bn_eval0 #t #0 res;
     assert_norm (pow2 0 = 1);
     bn_eval0 a;
     bn_eval0 b;
     () end
   else begin
-    let (c1, res1) : generate_elem_a uint64 carry aLen (i - 1) = generate_elems #uint64 #carry aLen (i - 1) (bn_add_f a b) (u64 0) in
-    generate_elems_unfold #uint64 #carry aLen i (bn_add_f a b) (u64 0) (i - 1);
-    assert (generate_elems #uint64 #carry aLen i (bn_add_f a b) (u64 0) ==
-      generate_elem_f aLen (bn_add_f a b) (i - 1) (generate_elems #uint64 #carry aLen (i - 1) (bn_add_f a b) (u64 0)));
-    assert ((c, res) == generate_elem_f #uint64 #carry aLen (bn_add_f a b) (i - 1) (c1, res1));
-    bn_add_lemma_loop #aLen a b (i - 1);
-    assert (v c1 * pow2 (64 * (i - 1)) + bn_v #(i - 1) res1 == eval_ aLen a (i - 1) + eval_ aLen b (i - 1));
-    bn_add_lemma_loop_step #aLen a b i (c1, res1);
-    assert (v c * pow2 (64 * i) + bn_v #i res == eval_ aLen a i + eval_ aLen b i);
+    let (c1, res1) : generate_elem_a (limb t) (carry t) aLen (i - 1) = generate_elems aLen (i - 1) (bn_add_f a b) (uint #t 0) in
+    generate_elems_unfold aLen i (bn_add_f a b) (uint #t 0) (i - 1);
+    assert (generate_elems aLen i (bn_add_f a b) (uint #t 0) ==
+      generate_elem_f aLen (bn_add_f a b) (i - 1) (generate_elems aLen (i - 1) (bn_add_f a b) (uint #t 0)));
+    assert ((c, res) == generate_elem_f aLen (bn_add_f a b) (i - 1) (c1, res1));
+    bn_add_lemma_loop a b (i - 1);
+    assert (v c1 * pow2 (p * (i - 1)) + bn_v #t #(i - 1) res1 == eval_ aLen a (i - 1) + eval_ aLen b (i - 1));
+    bn_add_lemma_loop_step a b i (c1, res1);
+    assert (v c * pow2 (p * i) + bn_v #t #i res == eval_ aLen a i + eval_ aLen b i);
     () end
 
 
 val bn_add_lemma:
-    #aLen:size_nat
+    #t:limb_t
+  -> #aLen:size_nat
   -> #bLen:size_nat{bLen <= aLen}
-  -> a:lbignum aLen
-  -> b:lbignum bLen -> Lemma
-  (let (c, res) = bn_add #aLen #bLen a b in
-   v c * pow2 (64 * aLen) + bn_v res == bn_v a + bn_v b)
+  -> a:lbignum t aLen
+  -> b:lbignum t bLen ->
+  Lemma (let (c, res) = bn_add a b in
+   v c * pow2 (bits t * aLen) + bn_v res == bn_v a + bn_v b)
 
-let bn_add_lemma #aLen #bLen a b =
-  let (c, res) = bn_add #aLen #bLen a b in
+let bn_add_lemma #t #aLen #bLen a b =
+  let p = bits t in
+  let (c, res) = bn_add a b in
   if bLen = aLen then
-    bn_add_lemma_loop #aLen a b aLen
+    bn_add_lemma_loop a b aLen
   else begin
     let a0 = sub a 0 bLen in
     let a1 = sub a bLen (aLen - bLen) in
 
-    let c0, res0 = generate_elems #uint64 #carry bLen bLen (bn_add_f a0 b) (u64 0) in
-    bn_add_lemma_loop #bLen a0 b bLen;
-    assert (v c0 * pow2 (64 * bLen) + bn_v #bLen res0 == eval_ bLen a0 bLen + eval_ bLen b bLen);
+    let c0, res0 = generate_elems bLen bLen (bn_add_f a0 b) (uint #t 0) in
+    bn_add_lemma_loop a0 b bLen;
+    assert (v c0 * pow2 (p * bLen) + bn_v #t #bLen res0 == eval_ bLen a0 bLen + eval_ bLen b bLen);
     let c1, res1 = bn_add1 a1 c0 in
     bn_add1_lemma a1 c0;
-    assert (v c1 * pow2 (64 * (aLen - bLen)) + bn_v res1 == bn_v a1 + v c0);
+    assert (v c1 * pow2 (p * (aLen - bLen)) + bn_v res1 == bn_v a1 + v c0);
     let res = concat #_ #bLen res0 res1 in
     eq_intro (slice res 0 bLen) res0;
     eq_intro (slice res bLen aLen) res1;
     bn_eval_split_i res bLen;
-    assert (bn_v res == bn_v #bLen res0 + pow2 (64 * bLen) * bn_v res1);
+    assert (bn_v res == bn_v #t #bLen res0 + pow2 (p * bLen) * bn_v res1);
     calc (==) {
-      bn_v #bLen res0 + pow2 (64 * bLen) * bn_v res1;
+      bn_v #t #bLen res0 + pow2 (p * bLen) * bn_v res1;
       (==) { }
-      eval_ bLen a0 bLen + eval_ bLen b bLen - v c0 * pow2 (64 * bLen) + pow2 (64 * bLen) * (bn_v a1 + v c0 - v c1 * pow2 (64 * (aLen - bLen)));
-      (==) { Math.Lemmas.distributivity_sub_right (pow2 (64 * bLen)) (bn_v a1 + v c0) (v c1 * pow2 (64 * (aLen - bLen))) }
-      eval_ bLen a0 bLen + eval_ bLen b bLen - v c0 * pow2 (64 * bLen) + pow2 (64 * bLen) * (bn_v a1 + v c0) - pow2 (64 * bLen) * v c1 * pow2 (64 * (aLen - bLen));
-      (==) { Math.Lemmas.paren_mul_right (pow2 (64 * bLen)) (v c1) (pow2 (64 * (aLen - bLen))); Math.Lemmas.pow2_plus (64 * bLen) (64 * (aLen - bLen)) }
-      eval_ bLen a0 bLen + eval_ bLen b bLen - v c0 * pow2 (64 * bLen) + pow2 (64 * bLen) * (bn_v a1 + v c0) - v c1 * pow2 (64 * aLen);
-      (==) { Math.Lemmas.distributivity_sub_right (pow2 (64 * bLen)) (bn_v a1) (v c0) }
-      eval_ bLen a0 bLen + eval_ bLen b bLen + pow2 (64 * bLen) * bn_v a1 - v c1 * pow2 (64 * aLen);
+      eval_ bLen a0 bLen + eval_ bLen b bLen - v c0 * pow2 (p * bLen) + pow2 (p * bLen) * (bn_v a1 + v c0 - v c1 * pow2 (p * (aLen - bLen)));
+      (==) { Math.Lemmas.distributivity_sub_right (pow2 (p * bLen)) (bn_v a1 + v c0) (v c1 * pow2 (p * (aLen - bLen))) }
+      eval_ bLen a0 bLen + eval_ bLen b bLen - v c0 * pow2 (p * bLen) + pow2 (p * bLen) * (bn_v a1 + v c0) - pow2 (p * bLen) * v c1 * pow2 (p * (aLen - bLen));
+      (==) { Math.Lemmas.paren_mul_right (pow2 (p * bLen)) (v c1) (pow2 (p * (aLen - bLen))); Math.Lemmas.pow2_plus (p * bLen) (p * (aLen - bLen)) }
+      eval_ bLen a0 bLen + eval_ bLen b bLen - v c0 * pow2 (p * bLen) + pow2 (p * bLen) * (bn_v a1 + v c0) - v c1 * pow2 (p * aLen);
+      (==) { Math.Lemmas.distributivity_sub_right (pow2 (p * bLen)) (bn_v a1) (v c0) }
+      eval_ bLen a0 bLen + eval_ bLen b bLen + pow2 (p * bLen) * bn_v a1 - v c1 * pow2 (p * aLen);
       (==) { bn_eval_split_i a bLen; bn_eval_extensionality_j a (sub a 0 bLen) bLen }
-      eval_ aLen a aLen + eval_ bLen b bLen  - v c1 * pow2 (64 * aLen);
+      eval_ aLen a aLen + eval_ bLen b bLen  - v c1 * pow2 (p * aLen);
     }; () end
 
 
 val bn_sub1_lemma_loop_step:
-    #aLen:size_nat
-  -> a:lbignum aLen
-  -> c_in:carry
+    #t:limb_t
+  -> #aLen:size_nat
+  -> a:lbignum t aLen
+  -> c_in:carry t
   -> i:pos{i <= aLen}
-  -> c1_res1:generate_elem_a uint64 carry aLen (i - 1)
-  -> Lemma
+  -> c1_res1:generate_elem_a (limb t) (carry t) aLen (i - 1) -> Lemma
   (requires
    (let (c1, res1) = c1_res1 in
-    bn_v #(i - 1) res1 - v c1 * pow2 (64 * (i - 1)) == eval_ aLen a (i - 1) - v c_in))
+    bn_v #t #(i - 1) res1 - v c1 * pow2 (bits t * (i - 1)) == eval_ aLen a (i - 1) - v c_in))
   (ensures
-   (let (c_out, res) = generate_elem_f #uint64 #carry aLen (bn_sub1_f a) (i - 1) c1_res1 in
-    bn_v #i res - v c_out * pow2 (64 * i) == eval_ aLen a i - v c_in))
+   (let (c_out, res) = generate_elem_f aLen (bn_sub1_f a) (i - 1) c1_res1 in
+    bn_v #t #i res - v c_out * pow2 (bits t * i) == eval_ aLen a i - v c_in))
 
-let bn_sub1_lemma_loop_step #aLen a c_in i (c1, res1) =
-  let (c_out, res) = generate_elem_f #uint64 #carry aLen (bn_sub1_f a) (i - 1) (c1, res1) in
+let bn_sub1_lemma_loop_step #t #aLen a c_in i (c1, res1) =
+  let p = bits t in
+  let (c_out, res) = generate_elem_f aLen (bn_sub1_f a) (i - 1) (c1, res1) in
   let c, e = bn_sub1_f a (i - 1) c1 in
-  assert (v e - v c * pow2 64 == v a.[i - 1] - v c1);
+  assert (v e - v c * pow2 p == v a.[i - 1] - v c1);
 
   calc (==) {
-    bn_v #i res - v c * pow2 (64 * i);
-    (==) { bn_eval_snoc #(i - 1) res1 e }
-    bn_v #(i - 1) res1 + v e * pow2 (64 * (i - 1)) - v c * pow2 (64 * i);
+    bn_v #t #i res - v c * pow2 (p * i);
+    (==) { bn_eval_snoc #t #(i - 1) res1 e }
+    bn_v #t #(i - 1) res1 + v e * pow2 (p * (i - 1)) - v c * pow2 (p * i);
     (==) { }
-    eval_ aLen a (i - 1) - v c_in + (v a.[i - 1] - v e + v c * pow2 64) * pow2 (64 * (i - 1)) + v e * pow2 (64 * (i - 1)) - v c * pow2 (64 * i);
-    (==) { Math.Lemmas.distributivity_sub_left (v a.[i - 1] + v c * pow2 64) (v e) (pow2 (64 * (i - 1))) }
-    eval_ aLen a (i - 1) - v c_in + (v a.[i - 1] + v c * pow2 64) * pow2 (64 * (i - 1)) - v c * pow2 (64 * i);
-    (==) { Math.Lemmas.distributivity_add_left (v a.[i - 1]) (v c * pow2 64) (pow2 (64 * (i - 1))) }
-    eval_ aLen a (i - 1) - v c_in + v a.[i - 1] * pow2 (64 * (i - 1)) + v c * pow2 64 * pow2 (64 * (i - 1)) - v c * pow2 (64 * i);
-    (==) { Math.Lemmas.paren_mul_right (v c) (pow2 64) (pow2 (64 * (i - 1))); Math.Lemmas.pow2_plus 64 (64 * (i - 1)) }
-    eval_ aLen a (i - 1) - v c_in + v a.[i - 1] * pow2 (64 * (i - 1));
-    (==) { bn_eval_unfold_i #aLen a i }
+    eval_ aLen a (i - 1) - v c_in + (v a.[i - 1] - v e + v c * pow2 p) * pow2 (p * (i - 1)) + v e * pow2 (p * (i - 1)) - v c * pow2 (p * i);
+    (==) { Math.Lemmas.distributivity_sub_left (v a.[i - 1] + v c * pow2 p) (v e) (pow2 (p * (i - 1))) }
+    eval_ aLen a (i - 1) - v c_in + (v a.[i - 1] + v c * pow2 p) * pow2 (p * (i - 1)) - v c * pow2 (p * i);
+    (==) { Math.Lemmas.distributivity_add_left (v a.[i - 1]) (v c * pow2 p) (pow2 (p * (i - 1))) }
+    eval_ aLen a (i - 1) - v c_in + v a.[i - 1] * pow2 (p * (i - 1)) + v c * pow2 p * pow2 (p * (i - 1)) - v c * pow2 (p * i);
+    (==) { Math.Lemmas.paren_mul_right (v c) (pow2 p) (pow2 (p * (i - 1))); Math.Lemmas.pow2_plus p (p * (i - 1)) }
+    eval_ aLen a (i - 1) - v c_in + v a.[i - 1] * pow2 (p * (i - 1));
+    (==) { bn_eval_unfold_i a i }
     eval_ aLen a i - v c_in;
   };
-  assert (bn_v #i res - v c * pow2 (64 * i) == eval_ aLen a i - v c_in)
+  assert (bn_v #t #i res - v c * pow2 (p * i) == eval_ aLen a i - v c_in)
 
 
 val bn_sub1_lemma_loop:
-    #aLen:size_nat
-  -> a:lbignum aLen
-  -> c_in:carry
-  -> i:nat{i <= aLen} -> Lemma
-  (let (c_out, res) : generate_elem_a uint64 carry aLen i = generate_elems #uint64 #carry aLen i (bn_sub1_f a) c_in in
-   bn_v #i res - v c_out * pow2 (64 * i) == eval_ aLen a i - v c_in)
+    #t:limb_t
+  -> #aLen:size_nat
+  -> a:lbignum t aLen
+  -> c_in:carry t
+  -> i:nat{i <= aLen} ->
+  Lemma (let (c_out, res) : generate_elem_a (limb t) (carry t) aLen i = generate_elems aLen i (bn_sub1_f a) c_in in
+   bn_v #t #i res - v c_out * pow2 (bits t * i) == eval_ aLen a i - v c_in)
 
-let rec bn_sub1_lemma_loop #aLen a c_in i =
-  let (c_out, res) : generate_elem_a uint64 carry aLen i = generate_elems #uint64 #carry aLen i (bn_sub1_f a) c_in in
+let rec bn_sub1_lemma_loop #t #aLen a c_in i =
+  let p = bits t in
+  let (c_out, res) : generate_elem_a (limb t) (carry t) aLen i = generate_elems aLen i (bn_sub1_f a) c_in in
   if i = 0 then begin
-    eq_generate_elems0 #uint64 #carry aLen i (bn_sub1_f a) c_in;
+    eq_generate_elems0  aLen i (bn_sub1_f a) c_in;
     assert (c_out == c_in /\ res == Seq.empty);
-    bn_eval0 #0 res;
+    bn_eval0 #t #0 res;
     assert_norm (pow2 0 = 1);
     bn_eval0 a;
     () end
   else begin
-    let (c1, res1) : generate_elem_a uint64 carry aLen (i - 1) = generate_elems #uint64 #carry aLen (i - 1) (bn_sub1_f a) c_in in
-    generate_elems_unfold #uint64 #carry aLen i (bn_sub1_f a) c_in (i - 1);
-    assert (generate_elems #uint64 #carry aLen i (bn_sub1_f a) c_in ==
-      generate_elem_f aLen (bn_sub1_f a) (i - 1) (generate_elems #uint64 #carry aLen (i - 1) (bn_sub1_f a) c_in));
-    assert ((c_out, res) == generate_elem_f #uint64 #carry aLen (bn_sub1_f a) (i - 1) (c1, res1));
-    bn_sub1_lemma_loop #aLen a c_in (i - 1);
-    assert (bn_v #(i - 1) res1 - v c1 * pow2 (64 * (i - 1)) == eval_ aLen a (i - 1) - v c_in);
-    bn_sub1_lemma_loop_step #aLen a c_in i (c1, res1);
-    assert (bn_v #i res - v c_out * pow2 (64 * i) == eval_ aLen a i - v c_in);
+    let (c1, res1) : generate_elem_a (limb t) (carry t) aLen (i - 1) = generate_elems aLen (i - 1) (bn_sub1_f a) c_in in
+    generate_elems_unfold aLen i (bn_sub1_f a) c_in (i - 1);
+    assert (generate_elems aLen i (bn_sub1_f a) c_in ==
+      generate_elem_f aLen (bn_sub1_f a) (i - 1) (generate_elems aLen (i - 1) (bn_sub1_f a) c_in));
+    assert ((c_out, res) == generate_elem_f  aLen (bn_sub1_f a) (i - 1) (c1, res1));
+    bn_sub1_lemma_loop a c_in (i - 1);
+    assert (bn_v #t #(i - 1) res1 - v c1 * pow2 (p * (i - 1)) == eval_ aLen a (i - 1) - v c_in);
+    bn_sub1_lemma_loop_step a c_in i (c1, res1);
+    assert (bn_v #t #i res - v c_out * pow2 (p * i) == eval_ aLen a i - v c_in);
     () end
 
-val bn_sub1_lemma: #aLen:size_nat -> a:lbignum aLen -> c_in:carry ->
-  Lemma
-  (let (c_out, res) = bn_sub1 #aLen a c_in in
-   bn_v res - v c_out * pow2 (64 * aLen) == bn_v a - v c_in)
 
-let bn_sub1_lemma #aLen a c_in =
-  let (c_out, res) = bn_sub1 #aLen a c_in in
-  bn_sub1_lemma_loop #aLen a c_in aLen
+val bn_sub1_lemma: #t:limb_t -> #aLen:size_nat -> a:lbignum t aLen -> c_in:carry t ->
+  Lemma (let (c_out, res) = bn_sub1 a c_in in
+   bn_v res - v c_out * pow2 (bits t * aLen) == bn_v a - v c_in)
+
+let bn_sub1_lemma #t #aLen a c_in =
+  let (c_out, res) = bn_sub1 a c_in in
+  bn_sub1_lemma_loop a c_in aLen
 
 
 val bn_sub_lemma_loop_step:
-    #aLen:size_nat
-  -> a:lbignum aLen
-  -> b:lbignum aLen
+   #t:limb_t
+  -> #aLen:size_nat
+  -> a:lbignum t aLen
+  -> b:lbignum t aLen
   -> i:pos{i <= aLen}
-  -> c1_res1:generate_elem_a uint64 carry aLen (i - 1)
-  -> Lemma
+  -> c1_res1:generate_elem_a (limb t) (carry t) aLen (i - 1) -> Lemma
   (requires
    (let (c1, res1) = c1_res1 in
-    bn_v #(i - 1) res1 - v c1 * pow2 (64 * (i - 1)) == eval_ aLen a (i - 1) - eval_ aLen b (i - 1)))
+    bn_v #t #(i - 1) res1 - v c1 * pow2 (bits t * (i - 1)) == eval_ aLen a (i - 1) - eval_ aLen b (i - 1)))
   (ensures
-   (let (c, res) = generate_elem_f #uint64 #carry aLen (bn_sub_f a b) (i - 1) c1_res1 in
-    bn_v #i res - v c * pow2 (64 * i) == eval_ aLen a i - eval_ aLen b i))
+   (let (c, res) = generate_elem_f aLen (bn_sub_f a b) (i - 1) c1_res1 in
+    bn_v #t #i res - v c * pow2 (bits t * i) == eval_ aLen a i - eval_ aLen b i))
 
-let bn_sub_lemma_loop_step #aLen a b i (c1, res1) =
-  let (c, res) = generate_elem_f #uint64 #carry aLen (bn_sub_f a b) (i - 1) (c1, res1) in
+let bn_sub_lemma_loop_step #t #aLen a b i (c1, res1) =
+  let p = bits t in
+  let (c, res) = generate_elem_f aLen (bn_sub_f a b) (i - 1) (c1, res1) in
   let c, e = bn_sub_f a b (i - 1) c1 in
-  assert (v e - v c * pow2 64 == v a.[i - 1] - v b.[i - 1] - v c1);
+  assert (v e - v c * pow2 p == v a.[i - 1] - v b.[i - 1] - v c1);
 
   calc (==) {
-    bn_v #i res - v c * pow2 (64 * i);
-    (==) { bn_eval_snoc #(i - 1) res1 e }
-    bn_v #(i - 1) res1 + v e * pow2 (64 * (i - 1)) - v c * pow2 (64 * i);
+    bn_v #t #i res - v c * pow2 (p * i);
+    (==) { bn_eval_snoc #t #(i - 1) res1 e }
+    bn_v #t #(i - 1) res1 + v e * pow2 (p * (i - 1)) - v c * pow2 (p * i);
     (==) { }
-    eval_ aLen a (i - 1) - eval_ aLen b (i - 1) + (v a.[i - 1] - v b.[i - 1] + v c * pow2 64 - v e) * pow2 (64 * (i - 1)) + v e * pow2 (64 * (i - 1)) - v c * pow2 (64 * i);
-    (==) { Math.Lemmas.distributivity_sub_left (v a.[i - 1] - v b.[i - 1] + v c * pow2 64) (v e) (pow2 (64 * (i - 1))) }
-    eval_ aLen a (i - 1) - eval_ aLen b (i - 1) + (v a.[i - 1] - v b.[i - 1] + v c * pow2 64) * pow2 (64 * (i - 1)) - v c * pow2 (64 * i);
-    (==) { Math.Lemmas.distributivity_add_left (v a.[i - 1] - v b.[i - 1]) (v c * pow2 64) (pow2 (64 * (i - 1))) }
-    eval_ aLen a (i - 1) - eval_ aLen b (i - 1) + (v a.[i - 1] - v b.[i - 1]) * pow2 (64 * (i - 1)) + v c * pow2 64 * pow2 (64 * (i - 1)) - v c * pow2 (64 * i);
-    (==) { Math.Lemmas.paren_mul_right (v c) (pow2 64) (pow2 (64 * (i - 1))); Math.Lemmas.pow2_plus 64 (64 * (i - 1)) }
-    eval_ aLen a (i - 1) - eval_ aLen b (i - 1) + (v a.[i - 1] - v b.[i - 1]) * pow2 (64 * (i - 1));
-    (==) { Math.Lemmas.distributivity_sub_left (v a.[i - 1]) (v b.[i - 1]) (pow2 (64 * (i - 1))) }
-    eval_ aLen a (i - 1) - eval_ aLen b (i - 1) + v a.[i - 1] * pow2 (64 * (i - 1)) - v b.[i - 1] * pow2 (64 * (i - 1));
-    (==) { bn_eval_unfold_i #aLen a i }
-    eval_ aLen a i - eval_ aLen b (i - 1) - v b.[i - 1] * pow2 (64 * (i - 1));
-    (==) { bn_eval_unfold_i #aLen b i }
+    eval_ aLen a (i - 1) - eval_ aLen b (i - 1) + (v a.[i - 1] - v b.[i - 1] + v c * pow2 p - v e) * pow2 (p * (i - 1)) + v e * pow2 (p * (i - 1)) - v c * pow2 (p * i);
+    (==) { Math.Lemmas.distributivity_sub_left (v a.[i - 1] - v b.[i - 1] + v c * pow2 p) (v e) (pow2 (p * (i - 1))) }
+    eval_ aLen a (i - 1) - eval_ aLen b (i - 1) + (v a.[i - 1] - v b.[i - 1] + v c * pow2 p) * pow2 (p * (i - 1)) - v c * pow2 (p * i);
+    (==) { Math.Lemmas.distributivity_add_left (v a.[i - 1] - v b.[i - 1]) (v c * pow2 p) (pow2 (p * (i - 1))) }
+    eval_ aLen a (i - 1) - eval_ aLen b (i - 1) + (v a.[i - 1] - v b.[i - 1]) * pow2 (p * (i - 1)) + v c * pow2 p * pow2 (p * (i - 1)) - v c * pow2 (p * i);
+    (==) { Math.Lemmas.paren_mul_right (v c) (pow2 p) (pow2 (p * (i - 1))); Math.Lemmas.pow2_plus p (p * (i - 1)) }
+    eval_ aLen a (i - 1) - eval_ aLen b (i - 1) + (v a.[i - 1] - v b.[i - 1]) * pow2 (p * (i - 1));
+    (==) { Math.Lemmas.distributivity_sub_left (v a.[i - 1]) (v b.[i - 1]) (pow2 (p * (i - 1))) }
+    eval_ aLen a (i - 1) - eval_ aLen b (i - 1) + v a.[i - 1] * pow2 (p * (i - 1)) - v b.[i - 1] * pow2 (p * (i - 1));
+    (==) { bn_eval_unfold_i a i }
+    eval_ aLen a i - eval_ aLen b (i - 1) - v b.[i - 1] * pow2 (p * (i - 1));
+    (==) { bn_eval_unfold_i b i }
     eval_ aLen a i - eval_ aLen b i;
   };
-  assert (bn_v #i res - v c * pow2 (64 * i) == eval_ aLen a i - eval_ aLen b i)
+  assert (bn_v #t #i res - v c * pow2 (p * i) == eval_ aLen a i - eval_ aLen b i)
 
 
 val bn_sub_lemma_loop:
-    #aLen:size_nat
-  -> a:lbignum aLen
-  -> b:lbignum aLen
-  -> i:nat{i <= aLen} -> Lemma
-  (let (c, res) : generate_elem_a uint64 carry aLen i = generate_elems #uint64 #carry aLen i (bn_sub_f a b) (u64 0) in
-   bn_v #i res - v c * pow2 (64 * i) == eval_ aLen a i - eval_ aLen b i)
+    #t:limb_t
+  -> #aLen:size_nat
+  -> a:lbignum t aLen
+  -> b:lbignum t aLen
+  -> i:nat{i <= aLen} ->
+  Lemma (let (c, res) : generate_elem_a (limb t) (carry t) aLen i = generate_elems aLen i (bn_sub_f a b) (uint #t 0) in
+   bn_v #t #i res - v c * pow2 (bits t * i) == eval_ aLen a i - eval_ aLen b i)
 
-let rec bn_sub_lemma_loop #aLen a b i =
-  let (c, res) : generate_elem_a uint64 carry aLen i = generate_elems #uint64 #carry aLen i (bn_sub_f a b) (u64 0) in
+let rec bn_sub_lemma_loop #t #aLen a b i =
+  let (c, res) : generate_elem_a (limb t) (carry t) aLen i = generate_elems aLen i (bn_sub_f a b) (uint #t 0) in
   if i = 0 then begin
-    eq_generate_elems0 #uint64 #carry aLen i (bn_sub_f a b) (u64 0);
-    assert (c == u64 0 /\ res == Seq.empty);
-    bn_eval0 #0 res;
+    eq_generate_elems0 aLen i (bn_sub_f a b) (uint #t 0);
+    assert (c == uint #t 0 /\ res == Seq.empty);
+    bn_eval0 #t #0 res;
     assert_norm (pow2 0 = 1);
     bn_eval0 a;
     bn_eval0 b;
     () end
   else begin
-    let (c1, res1) : generate_elem_a uint64 carry aLen (i - 1) = generate_elems #uint64 #carry aLen (i - 1) (bn_sub_f a b) (u64 0) in
-    generate_elems_unfold #uint64 #carry aLen i (bn_sub_f a b) (u64 0) (i - 1);
-    assert (generate_elems #uint64 #carry aLen i (bn_sub_f a b) (u64 0) ==
-      generate_elem_f aLen (bn_sub_f a b) (i - 1) (generate_elems #uint64 #carry aLen (i - 1) (bn_sub_f a b) (u64 0)));
-    assert ((c, res) == generate_elem_f #uint64 #carry aLen (bn_sub_f a b) (i - 1) (c1, res1));
-    bn_sub_lemma_loop #aLen a b (i - 1);
-    assert (bn_v #(i - 1) res1 - v c1 * pow2 (64 * (i - 1)) == eval_ aLen a (i - 1) - eval_ aLen b (i - 1));
-    bn_sub_lemma_loop_step #aLen a b i (c1, res1);
-    assert (bn_v #i res - v c * pow2 (64 * i) == eval_ aLen a i - eval_ aLen b i);
+    let (c1, res1) : generate_elem_a (limb t) (carry t) aLen (i - 1) = generate_elems aLen (i - 1) (bn_sub_f a b) (uint #t 0) in
+    generate_elems_unfold aLen i (bn_sub_f a b) (uint #t 0) (i - 1);
+    assert (generate_elems aLen i (bn_sub_f a b) (uint #t 0) ==
+      generate_elem_f aLen (bn_sub_f a b) (i - 1) (generate_elems aLen (i - 1) (bn_sub_f a b) (uint #t 0)));
+    assert ((c, res) == generate_elem_f aLen (bn_sub_f a b) (i - 1) (c1, res1));
+    bn_sub_lemma_loop a b (i - 1);
+    assert (bn_v #t #(i - 1) res1 - v c1 * pow2 (bits t * (i - 1)) == eval_ aLen a (i - 1) - eval_ aLen b (i - 1));
+    bn_sub_lemma_loop_step a b i (c1, res1);
+    assert (bn_v #t #i res - v c * pow2 (bits t * i) == eval_ aLen a i - eval_ aLen b i);
     () end
 
 
 val bn_sub_lemma:
-    #aLen:size_nat
+    #t:limb_t
+  -> #aLen:size_nat
   -> #bLen:size_nat{bLen <= aLen}
-  -> a:lbignum aLen
-  -> b:lbignum bLen -> Lemma
-  (let (c, res) = bn_sub #aLen #bLen a b in
-   bn_v res - v c * pow2 (64 * aLen) == bn_v a - bn_v b)
+  -> a:lbignum t aLen
+  -> b:lbignum t bLen ->
+  Lemma (let (c, res) = bn_sub a b in
+   bn_v res - v c * pow2 (bits t * aLen) == bn_v a - bn_v b)
 
-let bn_sub_lemma #aLen #bLen a b =
-  let (c, res) = bn_sub #aLen #bLen a b in
+let bn_sub_lemma #t #aLen #bLen a b =
+  let p = bits t in
+  let (c, res) = bn_sub a b in
   if bLen = aLen then
-    bn_sub_lemma_loop #aLen a b aLen
+    bn_sub_lemma_loop a b aLen
   else begin
     let a0 = sub a 0 bLen in
     let a1 = sub a bLen (aLen - bLen) in
 
-    let c0, res0 = generate_elems #uint64 #carry bLen bLen (bn_sub_f a0 b) (u64 0) in
-    bn_sub_lemma_loop #bLen a0 b bLen;
-    assert (bn_v #bLen res0 - v c0 * pow2 (64 * bLen) == eval_ bLen a0 bLen - eval_ bLen b bLen);
+    let c0, res0 = generate_elems bLen bLen (bn_sub_f a0 b) (uint #t 0) in
+    bn_sub_lemma_loop a0 b bLen;
+    assert (bn_v #t #bLen res0 - v c0 * pow2 (p * bLen) == eval_ bLen a0 bLen - eval_ bLen b bLen);
     let c1, res1 = bn_sub1 a1 c0 in
     bn_sub1_lemma a1 c0;
-    assert (bn_v res1 - v c1 * pow2 (64 * (aLen - bLen)) == bn_v a1 - v c0);
+    assert (bn_v res1 - v c1 * pow2 (p * (aLen - bLen)) == bn_v a1 - v c0);
     let res = concat #_ #bLen res0 res1 in
     eq_intro (slice res 0 bLen) res0;
     eq_intro (slice res bLen aLen) res1;
     bn_eval_split_i res bLen;
-    assert (bn_v res == bn_v #bLen res0 + pow2 (64 * bLen) * bn_v res1);
+    assert (bn_v res == bn_v #t #bLen res0 + pow2 (p * bLen) * bn_v res1);
     calc (==) {
-      bn_v #bLen res0 + pow2 (64 * bLen) * bn_v res1;
+      bn_v #t #bLen res0 + pow2 (p * bLen) * bn_v res1;
       (==) { }
-      eval_ bLen a0 bLen - eval_ bLen b bLen + v c0 * pow2 (64 * bLen) + pow2 (64 * bLen) * (bn_v a1 - v c0 + v c1 * pow2 (64 * (aLen - bLen)));
-      (==) { Math.Lemmas.distributivity_sub_right (pow2 (64 * bLen)) (bn_v a1 + v c1 * pow2 (64 * (aLen - bLen))) (v c0) }
-      eval_ bLen a0 bLen - eval_ bLen b bLen + v c0 * pow2 (64 * bLen) + pow2 (64 * bLen) * (bn_v a1 + v c1 * pow2 (64 * (aLen - bLen))) - pow2 (64 * bLen) * v c0;
-      (==) { Math.Lemmas.distributivity_add_right (pow2 (64 * bLen)) (bn_v a1) (v c1 * pow2 (64 * (aLen - bLen))) }
-      eval_ bLen a0 bLen - eval_ bLen b bLen + pow2 (64 * bLen) * bn_v a1 + pow2 (64 * bLen) * v c1 * pow2 (64 * (aLen - bLen));
-      (==) { Math.Lemmas.paren_mul_right (pow2 (64 * bLen)) (v c1) (pow2 (64 * (aLen - bLen))); Math.Lemmas.pow2_plus (64 * bLen) (64 * (aLen - bLen)) }
-      eval_ bLen a0 bLen - eval_ bLen b bLen + pow2 (64 * bLen) * bn_v a1 + v c1 * pow2 (64 * aLen);
+      eval_ bLen a0 bLen - eval_ bLen b bLen + v c0 * pow2 (p * bLen) + pow2 (p * bLen) * (bn_v a1 - v c0 + v c1 * pow2 (p * (aLen - bLen)));
+      (==) { Math.Lemmas.distributivity_sub_right (pow2 (p * bLen)) (bn_v a1 + v c1 * pow2 (p * (aLen - bLen))) (v c0) }
+      eval_ bLen a0 bLen - eval_ bLen b bLen + v c0 * pow2 (p * bLen) + pow2 (p * bLen) * (bn_v a1 + v c1 * pow2 (p * (aLen - bLen))) - pow2 (p * bLen) * v c0;
+      (==) { Math.Lemmas.distributivity_add_right (pow2 (p * bLen)) (bn_v a1) (v c1 * pow2 (p * (aLen - bLen))) }
+      eval_ bLen a0 bLen - eval_ bLen b bLen + pow2 (p * bLen) * bn_v a1 + pow2 (p * bLen) * v c1 * pow2 (p * (aLen - bLen));
+      (==) { Math.Lemmas.paren_mul_right (pow2 (p * bLen)) (v c1) (pow2 (p * (aLen - bLen))); Math.Lemmas.pow2_plus (p * bLen) (p * (aLen - bLen)) }
+      eval_ bLen a0 bLen - eval_ bLen b bLen + pow2 (p * bLen) * bn_v a1 + v c1 * pow2 (p * aLen);
       (==) { bn_eval_split_i a bLen; bn_eval_extensionality_j a (sub a 0 bLen) bLen }
-      eval_ aLen a aLen - eval_ bLen b bLen + v c1 * pow2 (64 * aLen);
+      eval_ aLen a aLen - eval_ bLen b bLen + v c1 * pow2 (p * aLen);
     }; () end
