code/bignum/Hacl.Spec.Bignum.Base.fst
@@ -4,63 +4,66 @@ open FStar.Mul
 open Lib.IntTypes
 open Lib.Sequence
 
+open Hacl.Spec.Bignum.Definitions
 
 #reset-options "--z3rlimit 50 --fuel 0 --ifuel 0"
 
 inline_for_extraction noextract
-let carry = x:uint64{uint_v x == 0 \/ uint_v x == 1}
+let carry (t:limb_t) = x:limb t{uint_v x == 0 \/ uint_v x == 1}
 
 (**
  This is non-stateful version of code/fallback functions
 *)
 inline_for_extraction noextract
-val addcarry_u64: c:carry -> a:uint64 -> b:uint64 ->
-  Pure (carry & uint64)
+val addcarry: #t:limb_t -> c:carry t -> a:limb t -> b:limb t ->
+  Pure (carry t & limb t)
   (requires True)
   (ensures  fun (c', r) ->
-    uint_v r + uint_v c' * pow2 64 == uint_v a + uint_v b + uint_v c)
+    uint_v r + uint_v c' * pow2 (bits t) == uint_v a + uint_v b + uint_v c)
 
-let addcarry_u64 cin x y =
+let addcarry #t cin x y =
   let res = x +. cin +. y in
-  let c = logand (logor (lt_mask res x) (logand (eq_mask res x) cin)) (u64 1) in
+  let c = logand (logor (lt_mask res x) (logand (eq_mask res x) cin)) (uint #t 1) in
   logand_lemma (eq_mask res x) cin;
   logor_lemma (lt_mask res x) (logand (eq_mask res x) cin);
-  logand_mask (logor (lt_mask res x) (logand (eq_mask res x) cin)) (u64 1) 1;
+  logand_mask (logor (lt_mask res x) (logand (eq_mask res x) cin)) (uint #t 1) 1;
   c, res
 
 
 inline_for_extraction noextract
-val subborrow_u64: c:carry -> a:uint64 -> b:uint64 ->
-  Pure (carry & uint64)
+val subborrow: #t:limb_t -> c:carry t -> a:limb t -> b:limb t ->
+  Pure (carry t & limb t)
   (requires True)
   (ensures  fun (c', r) ->
-    uint_v r - uint_v c' * pow2 64 == uint_v a - uint_v b - uint_v c)
+    uint_v r - uint_v c' * pow2 (bits t) == uint_v a - uint_v b - uint_v c)
 
-let subborrow_u64 cin x y =
+let subborrow #t cin x y =
   let res = x -. y -. cin in
-  let c = logand (logor (gt_mask res x) (logand (eq_mask res x) cin)) (u64 1) in
+  let c = logand (logor (gt_mask res x) (logand (eq_mask res x) cin)) (uint #t 1) in
   logand_lemma (eq_mask res x) cin;
   logor_lemma (gt_mask res x) (logand (eq_mask res x) cin);
-  logand_mask (logor (gt_mask res x) (logand (eq_mask res x) cin)) (u64 1) 1;
+  logand_mask (logor (gt_mask res x) (logand (eq_mask res x) cin)) (uint #t 1) 1;
   c, res
 
 
 
-let mask_values (#t:inttype{unsigned t}) (x:uint_t t SEC) =
+let mask_values (#t:limb_t) (x:limb t) =
   v x = v (zeros t SEC) \/ v x = v (ones t SEC)
 
 inline_for_extraction noextract
-let unsafe_bool_of_u64 (m:uint64) : b:bool{b <==> v m = v (ones U64 SEC)} =
+let unsafe_bool_of_limb (#t:limb_t) (m:limb t) : b:bool{b <==> v m = v (ones t SEC)} =
   let open Lib.RawIntTypes in
-  FStar.UInt64.(u64_to_UInt64 m =^ u64_to_UInt64 (ones U64 SEC))
+  match t with
+  | U32 -> FStar.UInt32.(u32_to_UInt32 m =^ u32_to_UInt32 (ones U32 SEC))
+  | U64 -> FStar.UInt64.(u64_to_UInt64 m =^ u64_to_UInt64 (ones U64 SEC))
 
 
 inline_for_extraction noextract
-val mask_select: #t:inttype{unsigned t} -> mask:uint_t t SEC -> a:uint_t t SEC -> b:uint_t t SEC -> uint_t t SEC
-let mask_select mask a b =
+val mask_select: #t:limb_t -> mask:limb t -> a:limb t -> b:limb t -> limb t
+let mask_select #t mask a b =
   (mask &. a) |. ((lognot mask) &. b)
 
-val mask_select_lemma: #t:inttype{unsigned t} -> mask:uint_t t SEC -> a:uint_t t SEC -> b:uint_t t SEC -> Lemma
+val mask_select_lemma: #t:limb_t -> mask:limb t -> a:limb t -> b:limb t -> Lemma
   (requires mask_values mask)
   (ensures  mask_select mask a b == (if v mask = 0 then b else a))
 
@@ -85,11 +88,11 @@ let mask_select_lemma #t mask a b =
     assert (v (mask_select mask a b) == v a) end
 
 
-val mask_select_lemma1: mask:uint64 -> a:uint64 -> b:uint64 -> Lemma
+val mask_select_lemma1: #t:limb_t -> mask:limb t -> a:limb t -> b:limb t -> Lemma
   (requires mask_values mask)
   (ensures  b ^. (mask &. (a ^. b)) == (if v mask = 0 then b else a))
 
-let mask_select_lemma1 mask a b =
+let mask_select_lemma1 #t mask a b =
   let t1 = mask &. (a ^. b) in
   let t2 = b ^. t1 in
   logand_lemma mask (a ^.b);
@@ -105,11 +108,11 @@ let mask_select_lemma1 mask a b =
     () end
 
 
-val lseq_mask_select_lemma: #len:size_nat ->a:lseq uint64 len -> b:lseq uint64 len -> mask:uint64 -> Lemma
+val lseq_mask_select_lemma: #t:limb_t -> #len:size_nat -> a:lseq (limb t) len -> b:lseq (limb t) len -> mask:limb t -> Lemma
   (requires mask_values mask)
   (ensures  map2 (mask_select mask) a b == (if v mask = 0 then b else a))
 
-let lseq_mask_select_lemma #len a b mask =
+let lseq_mask_select_lemma #t #len a b mask =
   let res = map2 (mask_select mask) a b in
 
   let lemma_aux (i:nat{i < len}) : Lemma (v res.[i] == (if v mask = 0 then v b.[i] else v a.[i])) =
