code/bignum/Hacl.Spec.Bignum.Convert.fst
@@ -11,76 +11,121 @@ open Hacl.Spec.Bignum.Definitions
 
 #reset-options "--z3rlimit 50 --fuel 0 --ifuel 0"
 
-val bn_from_uint: len:size_pos -> x:uint64 -> lbignum len
-let bn_from_uint len x =
-  let b = create len (u64 0) in
+val bn_from_uint: #t:limb_t -> len:size_pos -> x:limb t -> lbignum t len
+let bn_from_uint #t len x =
+  let b = create len (uint #t 0) in
   b.[0] <- x
 
-val bn_from_uint_lemma: len:size_pos -> x:uint64 ->
+val bn_from_uint_lemma: #t:limb_t -> len:size_pos -> x:limb t ->
   Lemma (bn_v (bn_from_uint len x) == uint_v x)
-let bn_from_uint_lemma len x =
-  let b = create len (u64 0) in
+
+let bn_from_uint_lemma #t len x =
+  let b = create len (uint #t 0) in
   let b = b.[0] <- x in
   bn_eval_split_i b 1;
-  assert (bn_v b == bn_v (slice b 0 1) + pow2 64 * bn_v (slice b 1 len));
-  eq_intro (slice b 1 len) (create (len - 1) (u64 0));
-  bn_eval_zeroes (len - 1) (len - 1);
+  assert (bn_v b == bn_v (slice b 0 1) + pow2 (bits t) * bn_v (slice b 1 len));
+  eq_intro (slice b 1 len) (create (len - 1) (uint #t 0));
+  bn_eval_zeroes #t (len - 1) (len - 1);
   assert (bn_v b == bn_v (slice b 0 1));
   bn_eval1 (slice b 0 1)
 
 
-val bn_from_bytes_be_f: len:size_nat{8 * len <= max_size_t} -> lseq uint8 (8 * len) -> i:nat{i < len} -> uint64
-let bn_from_bytes_be_f len b i =
-  uint_from_bytes_be (sub b ((len - i - 1) * 8) 8)
+val bn_from_bytes_be_f:
+    #t:limb_t
+  -> len:size_nat{numbytes t * len <= max_size_t}
+  -> lseq uint8 (numbytes t * len)
+  -> i:nat{i < len} ->
+  limb t
+
+let bn_from_bytes_be_f #t len b i =
+  uint_from_bytes_be (sub b ((len - i - 1) * numbytes t) (numbytes t))
 
 
-val bn_from_bytes_be_: len:size_nat{8 * len <= max_size_t} -> lseq uint8 (8 * len) -> lbignum len
-let bn_from_bytes_be_ len b = createi len (bn_from_bytes_be_f len b)
+val bn_from_bytes_be_:
+    #t:limb_t
+  -> len:size_nat{numbytes t * len <= max_size_t}
+  -> lseq uint8 (numbytes t * len) ->
+  lbignum t len
+
+let bn_from_bytes_be_ #t len b =
+  createi len (bn_from_bytes_be_f len b)
 
 
-val bn_from_bytes_be: len:size_pos{8 * blocks len 8 <= max_size_t} -> lseq uint8 len -> lbignum (blocks len 8)
-let bn_from_bytes_be len b =
-  let bnLen = blocks len 8 in
-  let tmpLen = 8 * bnLen in
+val bn_from_bytes_be:
+    #t:limb_t
+  -> len:size_pos{numbytes t * blocks len (numbytes t) <= max_size_t}
+  -> lseq uint8 len ->
+  lbignum t (blocks len (numbytes t))
+
+let bn_from_bytes_be #t len b =
+  let bnLen = blocks len (numbytes t) in
+  let tmpLen = numbytes t * bnLen in
   let tmp = create tmpLen (u8 0) in
   let tmp = update_sub tmp (tmpLen - len) len b in
   bn_from_bytes_be_ bnLen tmp
 
 
-val bn_from_bytes_le: len:size_pos{8 * blocks len 8 <= max_size_t} -> lseq uint8 len -> lbignum (blocks len 8)
-let bn_from_bytes_le len b =
-  let bnLen = blocks len 8 in
-  let tmpLen = 8 * bnLen in
+val bn_from_bytes_le:
+    #t:limb_t
+  -> len:size_pos{numbytes t * blocks len (numbytes t) <= max_size_t}
+  -> lseq uint8 len ->
+  lbignum t (blocks len (numbytes t))
+
+let bn_from_bytes_le #t len b =
+  let bnLen = blocks len (numbytes t) in
+  let tmpLen = numbytes t * bnLen in
   let tmp = create tmpLen (u8 0) in
   let tmp = update_sub tmp 0 len b in
   uints_from_bytes_le tmp
 
 
-val bn_to_bytes_be_f: len:size_nat{8 * len <= max_size_t} -> lbignum len -> i:nat{i < len} -> unit -> unit & lseq uint8 8
-let bn_to_bytes_be_f len b i () =
+val bn_to_bytes_be_f:
+    #t:limb_t
+  -> len:size_nat
+  -> lbignum t len
+  -> i:nat{i < len}
+  -> unit ->
+  unit & lseq uint8 (numbytes t)
+
+let bn_to_bytes_be_f #t len b i () =
   (), uint_to_bytes_be b.[len - i - 1]
 
 
-val bn_to_bytes_be_: len:size_nat{8 * len <= max_size_t} -> lbignum len -> lseq uint8 (8 * len)
-let bn_to_bytes_be_ len b =
+val bn_to_bytes_be_:
+    #t:limb_t
+  -> len:size_nat{numbytes t * len <= max_size_t}
+  -> lbignum t len ->
+  lseq uint8 (numbytes t * len)
+
+let bn_to_bytes_be_ #t len b =
   let a_spec (i:nat{i <= len}) = unit in
-  let _, o = generate_blocks 8 len len a_spec
+  let _, o = generate_blocks (numbytes t) len len a_spec
     (bn_to_bytes_be_f len b) () in
   o
 
 
-val bn_to_bytes_be: len:size_pos{8 * blocks len 8 <= max_size_t} -> lbignum (blocks len 8) -> lseq uint8 len
-let bn_to_bytes_be len b =
-  let bnLen = blocks len 8 in
-  let tmpLen = 8 * bnLen in
+val bn_to_bytes_be:
+    #t:limb_t
+  -> len:size_pos{numbytes t * blocks len (numbytes t) <= max_size_t}
+  -> lbignum t (blocks len (numbytes t)) ->
+  lseq uint8 len
+
+let bn_to_bytes_be #t len b =
+  let bnLen = blocks len (numbytes t) in
+  let tmpLen = numbytes t * bnLen in
   let tmp = bn_to_bytes_be_ bnLen b in
   sub tmp (tmpLen - len) len
 
 
-val bn_to_bytes_le: len:size_pos{8 * blocks len 8 <= max_size_t} -> lbignum (blocks len 8) -> lseq uint8 len
-let bn_to_bytes_le len b =
-  let bnLen = blocks len 8 in
-  let tmpLen = 8 * bnLen in
+val bn_to_bytes_le:
+    #t:limb_t
+  -> len:size_pos{numbytes t * blocks len (numbytes t) <= max_size_t}
+  -> lbignum t (blocks len (numbytes t)) ->
+  lseq uint8 len
+
+let bn_to_bytes_le #t len b =
+  let bnLen = blocks len (numbytes t) in
+  let tmpLen = numbytes t * bnLen in
   let tmp = uints_to_bytes_le b in
   sub tmp 0 len
 
@@ -88,68 +133,83 @@ let bn_to_bytes_le len b =
 ///  Lemmas
 ///
 
-val reverse: #len:size_nat -> b:lseq uint64 len -> lseq uint64 len
-let reverse #len b = createi len (fun i -> b.[len - i - 1])
+val reverse: #t:limb_t -> #len:size_nat -> b:lbignum t len -> lbignum t len
+let reverse #t #len b = createi len (fun i -> b.[len - i - 1])
 
-val twice_reverse: #len:size_nat -> b:lseq uint64 len -> Lemma (reverse (reverse b) == b)
-let twice_reverse #len b =
+
+val twice_reverse: #t:limb_t -> #len:size_nat -> b:lbignum t len -> Lemma (reverse (reverse b) == b)
+let twice_reverse #t #len b =
   let lemma_aux (i:nat{i < len}) : Lemma ((reverse (reverse b)).[i] == b.[i]) = () in
+
   Classical.forall_intro lemma_aux;
   eq_intro (reverse (reverse b)) b
 
-val reverse_slice1: #len:size_pos -> b:lseq uint64 len -> Lemma
-  (slice (reverse b) 1 len == reverse (slice b 0 (len - 1)))
-let reverse_slice1 #len b =
-  let lemma_aux (i:nat{i < len - 1}) : Lemma ((slice (reverse b) 1 len).[i] == (reverse (slice b 0 (len - 1))).[i]) =
-    () in
+
+val reverse_slice1: #t:limb_t -> #len:size_pos -> b:lbignum t len ->
+  Lemma (slice (reverse b) 1 len == reverse (slice b 0 (len - 1)))
+let reverse_slice1 #t #len b =
+  let lemma_aux (i:nat{i < len - 1}) :
+    Lemma ((slice (reverse b) 1 len).[i] == (reverse (slice b 0 (len - 1))).[i]) = () in
+
   Classical.forall_intro lemma_aux;
   eq_intro (slice (reverse b) 1 len) (reverse (slice b 0 (len - 1)))
 
 
-val bn_from_bytes_be_is_uints_from_bytes_be_reverse: len:size_nat{8 * len <= max_size_t} -> b:lseq uint8 (8 * len) -> Lemma
-  (bn_from_bytes_be_ len b == reverse (uints_from_bytes_be b))
-let bn_from_bytes_be_is_uints_from_bytes_be_reverse len b =
-  let lemma_aux (i:nat{i < len}) : Lemma ((bn_from_bytes_be_ len b).[i] == (reverse #len (uints_from_bytes_be b)).[i]) =
-    index_uints_from_bytes_be #U64 #SEC #len b (len - i - 1) in
+val bn_from_bytes_be_is_uints_from_bytes_be_reverse:
+    #t:limb_t
+  -> len:size_nat{numbytes t * len <= max_size_t}
+  -> b:lseq uint8 (numbytes t * len) ->
+  Lemma (bn_from_bytes_be_ len b == reverse (uints_from_bytes_be b))
+
+let bn_from_bytes_be_is_uints_from_bytes_be_reverse #t len b =
+  let lemma_aux (i:nat{i < len}) :
+    Lemma ((bn_from_bytes_be_ len b).[i] == (reverse #t #len (uints_from_bytes_be b)).[i])
+  =
+    index_uints_from_bytes_be #t #SEC #len b (len - i - 1) in
+
   Classical.forall_intro lemma_aux;
   eq_intro (bn_from_bytes_be_ len b) (reverse (uints_from_bytes_be b))
 
 
-val bn_v_is_nat_from_intseq_be_lemma: len:size_nat -> b:lseq uint64 len -> Lemma (bn_v b == nat_from_intseq_be (reverse b))
-let rec bn_v_is_nat_from_intseq_be_lemma len b =
+val bn_v_is_nat_from_intseq_be_lemma: #t:limb_t -> len:size_nat -> b:lbignum t len ->
+  Lemma (bn_v b == nat_from_intseq_be (reverse b))
+
+let rec bn_v_is_nat_from_intseq_be_lemma #t len b =
   if len = 0 then bn_eval0 b
   else begin
     let b1 = slice b 0 (len - 1) in
     bn_v_is_nat_from_intseq_be_lemma (len - 1) b1;
     assert (bn_v b1 == nat_from_intseq_be (reverse b1));
 
-    bn_eval_split_i #len b (len - 1);
-    //assert (bn_v b == bn_v b1 + pow2 (64 * (len - 1)) * bn_v (slice b (len - 1) len));
-    bn_eval_unfold_i #1 (slice b (len - 1) len) 1;
-    bn_eval0 #1 (slice b (len - 1) len);
+    bn_eval_split_i #t #len b (len - 1);
+    bn_eval_unfold_i #t #1 (slice b (len - 1) len) 1;
+    bn_eval0 #t #1 (slice b (len - 1) len);
     assert (bn_v (slice b (len - 1) len) == v b.[len - 1]);
-    assert (bn_v b == nat_from_intseq_be (reverse b1) + pow2 (64 * (len - 1)) * v b.[len - 1]);
+    assert (bn_v b == nat_from_intseq_be (reverse b1) + pow2 (bits t * (len - 1)) * v b.[len - 1]);
 
     nat_from_intseq_be_slice_lemma (reverse b) 1;
-    //assert (nat_from_intseq_be (reverse b) == nat_from_intseq_be (slice (reverse b) 1 len) + pow2 ((len - 1) * 64) * nat_from_intseq_be (slice (reverse b) 0 1));
-    reverse_slice1 #len b;
-    //assert (slice (reverse b) 1 len == reverse (slice b 0 (len - 1)));
-    //assert (nat_from_intseq_be (reverse b) == nat_from_intseq_be (reverse b1) + pow2 ((len - 1) * 64) * nat_from_intseq_be (slice (reverse b) 0 1));
+    reverse_slice1 #t #len b;
     assert ((reverse b).[0] == b.[len - 1]);
     nat_from_intseq_be_lemma0 (slice (reverse b) 0 1);
     assert (nat_from_intseq_be (slice (reverse b) 0 1) == v b.[len - 1]);
     assert  (bn_v b == nat_from_intseq_be (reverse b));
     () end
 
-val bn_from_bytes_be_lemma_: len:size_nat{8 * len <= max_size_t} -> b:lseq uint8 (8 * len) -> Lemma
-  (bn_v (bn_from_bytes_be_ len b) == nat_from_bytes_be b)
-let bn_from_bytes_be_lemma_ len b =
+
+val bn_from_bytes_be_lemma_:
+    #t:limb_t
+  -> len:size_nat{numbytes t * len <= max_size_t}
+  -> b:lseq uint8 (numbytes t * len) ->
+  Lemma (bn_v (bn_from_bytes_be_ len b) == nat_from_bytes_be b)
+
+let bn_from_bytes_be_lemma_ #t len b =
   bn_v_is_nat_from_intseq_be_lemma len (bn_from_bytes_be_ len b);
   bn_from_bytes_be_is_uints_from_bytes_be_reverse len b;
-  twice_reverse (uints_from_bytes_be #U64 #SEC #len b);
-  assert (bn_v (bn_from_bytes_be_ len b) == nat_from_intseq_be (uints_from_bytes_be #U64 #SEC #len b));
-  uints_from_bytes_be_nat_lemma #U64 #SEC #len b;
-  assert (nat_from_intseq_be (uints_from_bytes_be #U64 #SEC #len b) == nat_from_bytes_be b)
+  twice_reverse (uints_from_bytes_be #t #SEC #len b);
+  assert (bn_v (bn_from_bytes_be_ len b) == nat_from_intseq_be (uints_from_bytes_be #t #SEC #len b));
+  uints_from_bytes_be_nat_lemma #t #SEC #len b;
+  assert (nat_from_intseq_be (uints_from_bytes_be #t #SEC #len b) == nat_from_bytes_be b)
+
 
 val lemma_nat_from_bytes_be_zeroes: len:size_nat -> b:lseq uint8 len -> Lemma
   (requires (forall (i:nat). i < len ==> b.[i] == u8 0))
@@ -163,9 +223,9 @@ let rec lemma_nat_from_bytes_be_zeroes len b =
     lemma_nat_from_bytes_be_zeroes (len-1) (slice b 1 len) end
 
 
-val nat_from_bytes_be_eq_lemma: len0:size_nat -> len:size_nat{len0 <= len} -> b:lseq uint8 len0 -> Lemma
- (let tmp = create len (u8 0) in
-  nat_from_intseq_be b == nat_from_intseq_be (update_sub tmp (len - len0) len0 b))
+val nat_from_bytes_be_eq_lemma: len0:size_nat -> len:size_nat{len0 <= len} -> b:lseq uint8 len0 ->
+  Lemma (let tmp = create len (u8 0) in
+    nat_from_intseq_be b == nat_from_intseq_be (update_sub tmp (len - len0) len0 b))
 
 let nat_from_bytes_be_eq_lemma len0 len b =
   let tmp = create len (u8 0) in
@@ -178,90 +238,125 @@ let nat_from_bytes_be_eq_lemma len0 len b =
   lemma_nat_from_bytes_be_zeroes (len - len0) (Seq.slice r 0 (len - len0))
 
 
-val bn_from_bytes_be_lemma: len:size_pos{8 * blocks len 8 <= max_size_t} -> b:lseq uint8 len -> Lemma
-  (bn_v (bn_from_bytes_be len b) == nat_from_bytes_be b)
-let bn_from_bytes_be_lemma len b =
-  let bnLen = blocks len 8 in
-  let tmpLen = 8 * bnLen in
+val bn_from_bytes_be_lemma:
+    #t:limb_t
+  -> len:size_pos{numbytes t * blocks len (numbytes t) <= max_size_t}
+  -> b:lseq uint8 len ->
+  Lemma (bn_v (bn_from_bytes_be #t len b) == nat_from_bytes_be b)
+
+let bn_from_bytes_be_lemma #t len b =
+  let bnLen = blocks len (numbytes t) in
+  let tmpLen = numbytes t * bnLen in
   let tmp = create tmpLen (u8 0) in
   let tmp = update_sub tmp (tmpLen - len) len b in
-  let res = bn_from_bytes_be_ bnLen tmp in
-  bn_from_bytes_be_lemma_ bnLen tmp;
-  assert (bn_v (bn_from_bytes_be_ bnLen tmp) == nat_from_bytes_be tmp);
+  let res = bn_from_bytes_be_ #t bnLen tmp in
+  bn_from_bytes_be_lemma_ #t bnLen tmp;
+  assert (bn_v (bn_from_bytes_be_ #t bnLen tmp) == nat_from_bytes_be tmp);
   nat_from_bytes_be_eq_lemma len tmpLen b
 
-val index_bn_to_bytes_be_: len:size_nat{8 * len <= max_size_t} -> b:lbignum len -> i:nat{i < 8 * len} ->
-  Lemma ((bn_to_bytes_be_ len b).[i] == uint #U8 #SEC (v b.[len - i / 8 - 1] / pow2 (8 * (7 - i % 8)) % pow2 8))
-let index_bn_to_bytes_be_ len b i =
-  let bi = b.[len - i / 8 - 1] in
-  index_generate_blocks 8 len len (bn_to_bytes_be_f len b) i;
-  assert ((bn_to_bytes_be_ len b).[i] == (uint_to_bytes_be bi).[i % 8]);
-  index_uint_to_bytes_be bi;
-  assert ((uint_to_bytes_be bi).[i % 8] == uint #U8 #SEC (v bi / pow2 (8 * (7 - i % 8)) % pow2 8))
 
-val bn_to_bytes_be_lemma_aux: len:size_pos{8 * len <= max_size_t} -> b:lbignum len{bn_v b < pow2 (64 * len)} -> i:nat{i < 8 * len} -> Lemma
-  (bn_v b / pow2 (8 * (8 * len - i - 1)) % pow2 8 == v b.[len - i / 8 - 1] / pow2 (8 * (7 - i % 8)) % pow2 8)
-let bn_to_bytes_be_lemma_aux len b i =
+val index_bn_to_bytes_be_:
+    #t:limb_t
+  -> len:size_nat{numbytes t * len <= max_size_t}
+  -> b:lbignum t len
+  -> i:nat{i < numbytes t * len} ->
+  Lemma (let numb = numbytes t in
+    (bn_to_bytes_be_ #t len b).[i] ==
+    uint #U8 #SEC (v b.[len - i / numb - 1] / pow2 (8 * (numb - 1 - i % numb)) % pow2 8))
+
+let index_bn_to_bytes_be_ #t len b i =
+  let numb = numbytes t in
+  let bi = b.[len - i / numb - 1] in
+  index_generate_blocks (numb) len len (bn_to_bytes_be_f len b) i;
+  assert ((bn_to_bytes_be_ #t len b).[i] == (uint_to_bytes_be bi).[i % numb]);
+  index_uint_to_bytes_be bi;
+  assert ((uint_to_bytes_be bi).[i % numb] == uint #U8 #SEC (v bi / pow2 (8 * (numb - 1 - i % numb)) % pow2 8))
+
+
+val bn_to_bytes_be_lemma_aux:
+    #t:limb_t
+  -> len:size_pos{numbytes t * len <= max_size_t}
+  -> b:lbignum t len{bn_v b < pow2 (bits t * len)}
+  -> i:nat{i < numbytes t * len} ->
+  Lemma (let numb = numbytes t in
+    bn_v b / pow2 (8 * (numb * len - i - 1)) % pow2 8 ==
+    v b.[len - i / numb - 1] / pow2 (8 * (numb - 1 - i % numb)) % pow2 8)
+
+let bn_to_bytes_be_lemma_aux #t len b i =
+  let numb = numbytes t in
+  let p = pow2 8 in
+  let e  = numb - 1 - i % numb in
+  let e1 = len - i / numb - 1 in
+  let e2 = numb * len - 1 - i in
+
   calc (==) {
-    v b.[len - i / 8 - 1] / pow2 (8 * (7 - i % 8)) % pow2 8;
-    (==) { bn_eval_index b (len - i / 8 - 1) }
-    (bn_v b / pow2 (64 * (len - i / 8 - 1)) % pow2 64) / pow2 (8 * (7 - i % 8)) % pow2 8;
-    (==) { Math.Lemmas.pow2_modulo_division_lemma_1 (bn_v b) (64 * (len - i / 8 - 1)) (64 + 64 * (len - i / 8 - 1)) }
-    (bn_v b % pow2 (64 + 64 * (len - i / 8 - 1)) / pow2 (64 * (len - i / 8 - 1))) / pow2 (8 * (7 - i % 8)) % pow2 8;
-    (==) { Math.Lemmas.division_multiplication_lemma (bn_v b % pow2 (64 + 64 * (len - i / 8 - 1))) (pow2 (64 * (len - i / 8 - 1))) (pow2 (8 * (7 - i % 8))) }
-    (bn_v b % pow2 (64 + 64 * (len - i / 8 - 1))) / (pow2 (64 * (len - i / 8 - 1)) * pow2 (8 * (7 - i % 8))) % pow2 8;
-    (==) { Math.Lemmas.pow2_plus (64 * (len - i / 8 - 1)) (8 * (7 - i % 8)) }
-    (bn_v b % pow2 (64 + 64 * (len - i / 8 - 1))) / pow2 (64 * (len - i / 8 - 1) + 8 * (7 - i % 8)) % pow2 8;
-    (==) { Math.Lemmas.paren_mul_right 8 8 (len - i / 8 - 1);
-      Math.Lemmas.distributivity_add_right 8 (8 * (len - i / 8 - 1)) (7 - i % 8) }
-    (bn_v b % pow2 (64 + 64 * (len - i / 8 - 1))) / pow2 (8 * (8 * (len - 1 - i / 8) + 7 - i % 8)) % pow2 8;
-    (==) { Math.Lemmas.distributivity_sub_right 8 (len - 1) (i / 8); Math.Lemmas.euclidean_division_definition i 8 }
-    (bn_v b % pow2 (64 + 64 * (len - i / 8 - 1))) / pow2 (8 * (8 * (len - 1) - i + 7)) % pow2 8;
-    (==) { Math.Lemmas.distributivity_sub_right 8 len 1 }
-    (bn_v b % pow2 (64 + 64 * (len - i / 8 - 1))) / pow2 (8 * (8 * len - 1 - i)) % pow2 8;
-    (==) { Math.Lemmas.pow2_modulo_division_lemma_1 (bn_v b) (8 * (8 * len - 1 - i)) (64 + 64 * (len - i / 8 - 1)) }
-    (bn_v b / pow2 (8 * (8 * len - 1 - i))) % pow2 (64 + 64 * (len - i / 8 - 1) - 8 * (8 * len - 1 - i)) % pow2 8;
-    (==) { Math.Lemmas.pow2_modulo_modulo_lemma_1 (bn_v b / pow2 (8 * (8 * len - 1 - i))) 8 (64 + 64 * (len - i / 8 - 1) - 8 * (8 * len - 1 - i)) }
-    (bn_v b / pow2 (8 * (8 * len - i - 1))) % pow2 8;
+    v b.[e1] / pow2 (8 * e) % p;
+    (==) { bn_eval_index b e1 }
+    (bn_v b / pow2 (bits t * e1) % pow2 (bits t)) / pow2 (8 * e) % p;
+    (==) { Math.Lemmas.pow2_modulo_division_lemma_1 (bn_v b) (bits t * e1) (bits t + bits t * e1) }
+    (bn_v b % pow2 (bits t + bits t * e1) / pow2 (bits t * e1)) / pow2 (8 * e) % p;
+    (==) { Math.Lemmas.division_multiplication_lemma (bn_v b % pow2 (bits t + bits t * e1)) (pow2 (bits t * e1)) (pow2 (8 * e)) }
+    (bn_v b % pow2 (bits t + bits t * e1)) / (pow2 (bits t * e1) * pow2 (8 * e)) % p;
+    (==) { Math.Lemmas.pow2_plus (bits t * e1) (8 * e) }
+    (bn_v b % pow2 (bits t + bits t * e1)) / pow2 (bits t * e1 + 8 * e) % p;
+    (==) { Math.Lemmas.pow2_modulo_division_lemma_1 (bn_v b) (8 * e2) (bits t + bits t * e1) }
+    (bn_v b / pow2 (8 * e2)) % pow2 (bits t + bits t * e1 - 8 * e2) % p;
+    (==) { Math.Lemmas.pow2_modulo_modulo_lemma_1 (bn_v b / pow2 (8 * e2)) 8 (bits t + bits t * e1 - 8 * e2) }
+    (bn_v b / pow2 (8 * (numb * len - i - 1))) % p;
     }
 
-val bn_to_bytes_be_lemma_: len:size_pos{8 * len <= max_size_t} -> b:lbignum len{bn_v b < pow2 (64 * len)} -> Lemma
-  (bn_to_bytes_be_ len b == nat_to_intseq_be #U8 #SEC (8 * len) (bn_v b))
-let bn_to_bytes_be_lemma_ len b =
-  let lemma_aux (i:nat{i < 8 * len}) : Lemma ((bn_to_bytes_be_ len b).[i] == index #uint8 #(8 * len) (nat_to_intseq_be (8 * len) (bn_v b)) i) =
-    let rp = nat_to_intseq_be #U8 #SEC (8 * len) (bn_v b) in
-    index_nat_to_intseq_be #U8 #SEC (8 * len) (bn_v b) (8 * len - i - 1);
-    //assert (index #uint8 #(8 * len) rp i == uint #U8 #SEC (bn_v b / pow2 (8 * (8 * len - i - 1)) % pow2 8));
+
+val bn_to_bytes_be_lemma_:
+    #t:limb_t
+  -> len:size_pos{numbytes t * len <= max_size_t}
+  -> b:lbignum t len{bn_v b < pow2 (bits t * len)} ->
+  Lemma (bn_to_bytes_be_ #t len b == nat_to_intseq_be #U8 #SEC (numbytes t * len) (bn_v b))
+
+let bn_to_bytes_be_lemma_ #t len b =
+  let numb = numbytes t in
+
+  let lemma_aux (i:nat{i < numb * len}) :
+    Lemma ((bn_to_bytes_be_ #t len b).[i] == index #uint8 #(numb * len) (nat_to_intseq_be (numb * len) (bn_v b)) i)
+  =
+    let rp = nat_to_intseq_be #U8 #SEC (numb * len) (bn_v b) in
+    index_nat_to_intseq_be #U8 #SEC (numb * len) (bn_v b) (numb * len - i - 1);
+    assert (index #uint8 #(numb * len) rp i == uint #U8 #SEC (bn_v b / pow2 (8 * (numb * len - i - 1)) % pow2 8));
     index_bn_to_bytes_be_ len b i;
-    //assert ((bn_to_bytes_be_ len b).[i] == uint #U8 #SEC (v b.[len - i / 8 - 1] / pow2 (8 * (7 - i % 8)) % pow2 8));
+    assert ((bn_to_bytes_be_ #t len b).[i] == uint #U8 #SEC (v b.[len - i / numb - 1] / pow2 (8 * (numb - 1 - i % numb)) % pow2 8));
     bn_to_bytes_be_lemma_aux len b i;
     () in
-  Classical.forall_intro lemma_aux;
-  eq_intro (bn_to_bytes_be_ len b) (nat_to_intseq_be (8 * len) (bn_v b))
 
-val bn_to_bytes_be_lemma: len:size_pos{8 * blocks len 8 <= max_size_t} -> b:lbignum (blocks len 8){bn_v b < pow2 (8 * len)} -> Lemma
-  (bn_to_bytes_be len b == nat_to_intseq_be #U8 #SEC len (bn_v b))
-let bn_to_bytes_be_lemma len b =
-  let bnLen = blocks len 8 in
-  let tmpLen = 8 * bnLen in
+  Classical.forall_intro lemma_aux;
+  eq_intro (bn_to_bytes_be_ len b) (nat_to_intseq_be (numb * len) (bn_v b))
+
+
+val bn_to_bytes_be_lemma:
+    #t:limb_t
+  -> len:size_pos{numbytes t * blocks len (numbytes t) <= max_size_t}
+  -> b:lbignum t (blocks len (numbytes t)){bn_v b < pow2 (8 * len)} ->
+  Lemma (bn_to_bytes_be #t len b == nat_to_intseq_be #U8 #SEC len (bn_v b))
+
+let bn_to_bytes_be_lemma #t len b =
+  let bnLen = blocks len (numbytes t) in
+  let tmpLen = numbytes t * bnLen in
   let tmp = bn_to_bytes_be_ bnLen b in
   let res = sub tmp (tmpLen - len) len in
   assert (bn_v b < pow2 (8 * len));
-  Math.Lemmas.pow2_le_compat (64 * bnLen) (8 * len);
-  assert (bn_v b < pow2 (64 * bnLen));
+  Math.Lemmas.pow2_le_compat (bits t * bnLen) (8 * len);
+  assert (bn_v b < pow2 (bits t * bnLen));
   bn_to_bytes_be_lemma_ bnLen b;
-  assert (tmp == nat_to_intseq_be #U8 #SEC (8 * bnLen) (bn_v b));
+  assert (tmp == nat_to_intseq_be #U8 #SEC tmpLen (bn_v b));
 
   let lemma_aux (i:nat{i < len}) :
-    Lemma (index (sub #uint8 #(8 * bnLen) (nat_to_intseq_be #U8 #SEC (8 * bnLen) (bn_v b)) (tmpLen - len) len) i ==
+    Lemma (index (sub #uint8 #tmpLen (nat_to_intseq_be #U8 #SEC tmpLen (bn_v b)) (tmpLen - len) len) i ==
            index #uint8 #len (nat_to_intseq_be #U8 #SEC len (bn_v b)) i) =
     let rp = nat_to_intseq_be #U8 #SEC len (bn_v b) in
     index_nat_to_intseq_be #U8 #SEC len (bn_v b) (len - i - 1);
     assert (index #uint8 #len rp i == uint #U8 #SEC (bn_v b / pow2 (8 * (len - i - 1)) % pow2 8));
-    let lp = nat_to_intseq_be #U8 #SEC (8 * bnLen) (bn_v b) in
-    assert (index (sub #uint8 #(8 * bnLen) lp (tmpLen - len) len) i == index #uint8 #(8 * bnLen) lp (tmpLen - len + i));
-    index_nat_to_intseq_be #U8 #SEC (8 * bnLen) (bn_v b) (len - i - 1);
-    assert (index #uint8 #(8 * bnLen) lp (tmpLen - len + i) == uint #U8 #SEC (bn_v b / pow2 (8 * (len - i - 1)) % pow2 8));
+    let lp = nat_to_intseq_be #U8 #SEC tmpLen (bn_v b) in
+    assert (index (sub #uint8 #tmpLen lp (tmpLen - len) len) i == index #uint8 #tmpLen lp (tmpLen - len + i));
+    index_nat_to_intseq_be #U8 #SEC tmpLen (bn_v b) (len - i - 1);
+    assert (index #uint8 #tmpLen lp (tmpLen - len + i) == uint #U8 #SEC (bn_v b / pow2 (8 * (len - i - 1)) % pow2 8));
     () in
 
   Classical.forall_intro lemma_aux;
@@ -270,8 +365,10 @@ let bn_to_bytes_be_lemma len b =
 
 (* Little-endian *)
 
-val bn_v_is_nat_from_intseq_le_lemma: len:size_nat -> b:lseq uint64 len -> Lemma (bn_v b == nat_from_intseq_le b)
-let rec bn_v_is_nat_from_intseq_le_lemma len b =
+val bn_v_is_nat_from_intseq_le_lemma: #t:limb_t -> len:size_nat -> b:lbignum t len ->
+  Lemma (bn_v b == nat_from_intseq_le b)
+
+let rec bn_v_is_nat_from_intseq_le_lemma #t len b =
   if len = 0 then
     bn_eval0 b
   else begin
@@ -279,16 +376,13 @@ let rec bn_v_is_nat_from_intseq_le_lemma len b =
     bn_v_is_nat_from_intseq_le_lemma (len - 1) b1;
     assert (bn_v b1 == nat_from_intseq_le b1);
 
-    bn_eval_split_i #len b (len - 1);
-    //assert (bn_v b == bn_v b1 + pow2 (64 * (len - 1)) * bn_v (slice b (len - 1) len));
-    bn_eval_unfold_i #1 (slice b (len - 1) len) 1;
-    bn_eval0 #1 (slice b (len - 1) len);
-    //assert (bn_v (slice b (len - 1) len) == v b.[len - 1]);
-    assert (bn_v b == nat_from_intseq_le b1 + pow2 (64 * (len - 1)) * v b.[len - 1]);
+    bn_eval_split_i #t #len b (len - 1);
+    bn_eval_unfold_i #t #1 (slice b (len - 1) len) 1;
+    bn_eval0 #t #1 (slice b (len - 1) len);
+    assert (bn_v b == nat_from_intseq_le b1 + pow2 (bits t * (len - 1)) * v b.[len - 1]);
     nat_from_intseq_le_slice_lemma b (len - 1);
-    //assert (nat_from_intseq_le b == nat_from_intseq_le b1 + pow2 ((len - 1) * 64) * nat_from_intseq_le (slice b (len - 1) len));
     nat_from_intseq_le_lemma0 (slice b (len - 1) len);
-    assert (nat_from_intseq_le b == nat_from_intseq_le b1 + pow2 ((len - 1) * 64) * v b.[len - 1]) end
+    assert (nat_from_intseq_le b == nat_from_intseq_le b1 + pow2 ((len - 1) * bits t) * v b.[len - 1]) end
 
 
 val lemma_nat_from_bytes_le_zeroes: len:size_nat -> b:lseq uint8 len -> Lemma
@@ -318,46 +412,47 @@ let nat_from_bytes_le_eq_lemma len0 len b =
   lemma_nat_from_bytes_le_zeroes (len - len0) (Seq.slice r len0 len)
 
 
-val bn_from_bytes_le_lemma: len:size_pos{8 * (blocks len 8) <= max_size_t} -> b:lseq uint8 len ->
-  Lemma (bn_v (bn_from_bytes_le len b) == nat_from_bytes_le b)
-let bn_from_bytes_le_lemma len b =
-  let bnLen = blocks len 8 in
-  let tmpLen = 8 * bnLen in
+val bn_from_bytes_le_lemma:
+    #t:limb_t
+  -> len:size_pos{numbytes t * (blocks len (numbytes t)) <= max_size_t}
+  -> b:lseq uint8 len ->
+  Lemma (bn_v (bn_from_bytes_le #t len b) == nat_from_bytes_le b)
+
+let bn_from_bytes_le_lemma #t len b =
+  let bnLen = blocks len (numbytes t) in
+  let tmpLen = numbytes t * bnLen in
   let tmp = create tmpLen (u8 0) in
   let tmp = update_sub tmp 0 len b in
-  let res = uints_from_bytes_le #U64 #SEC #bnLen tmp in
-  uints_from_bytes_le_nat_lemma #U64 #SEC #bnLen tmp;
-  //assert (nat_from_intseq_le res == nat_from_intseq_le tmp);
+  let res = uints_from_bytes_le #t #SEC #bnLen tmp in
+  uints_from_bytes_le_nat_lemma #t #SEC #bnLen tmp;
   bn_v_is_nat_from_intseq_le_lemma bnLen res;
-  //assert (bn_v res == nat_from_intseq_le res);
   nat_from_bytes_le_eq_lemma len tmpLen b
-  //assert (nat_from_intseq_le tmp == nat_from_intseq_le b)
 
 
 val bn_to_bytes_le_lemma:
-    len:size_pos{8 * (blocks len 8) <= max_size_t}
-  -> b:lbignum (blocks len 8){bn_v b < pow2 (8 * len)} ->
+    #t:limb_t
+  -> len:size_pos{numbytes t * (blocks len (numbytes t)) <= max_size_t}
+  -> b:lbignum t (blocks len (numbytes t)){bn_v b < pow2 (8 * len)} ->
   Lemma (bn_to_bytes_le len b == nat_to_intseq_le #U8 len (bn_v b))
-let bn_to_bytes_le_lemma len b =
-  let bnLen = blocks len 8 in
-  let tmpLen = 8 * bnLen in
+
+let bn_to_bytes_le_lemma #t len b =
+  let bnLen = blocks len (numbytes t) in
+  let tmpLen = numbytes t * bnLen in
   let tmp = uints_to_bytes_le b in
   let res = sub tmp 0 len in
   assert (bn_v b < pow2 (8 * len));
-  Math.Lemmas.pow2_le_compat (64 * bnLen) (8 * len);
-  assert (bn_v b < pow2 (64 * bnLen));
+  Math.Lemmas.pow2_le_compat (bits t * bnLen) (8 * len);
+  assert (bn_v b < pow2 (bits t * bnLen));
 
-  uints_to_bytes_le_nat_lemma #U64 #SEC bnLen (bn_v b);
-  //assert (uints_to_bytes_le #U64 #SEC #bnLen (nat_to_intseq_le #U64 #SEC bnLen (bn_v b)) == nat_to_bytes_le (bnLen * 8) (bn_v b));
+  uints_to_bytes_le_nat_lemma #t #SEC bnLen (bn_v b);
   bn_v_is_nat_from_intseq_le_lemma bnLen b;
   lemma_nat_from_to_intseq_le_preserves_value bnLen b;
-  //assert (nat_to_intseq_le #U64 #SEC bnLen (bn_v b) == b);
-  assert (uints_to_bytes_le #U64 #SEC #bnLen b == nat_to_intseq_le #U8 (bnLen * 8) (bn_v b));
+  assert (uints_to_bytes_le #t #SEC #bnLen b == nat_to_intseq_le #U8 tmpLen (bn_v b));
 
   let aux (i:nat{i < len}) :
-    Lemma (index #uint8 #tmpLen (nat_to_intseq_le #U8 (bnLen * 8) (bn_v b)) i ==
+    Lemma (index #uint8 #tmpLen (nat_to_intseq_le #U8 tmpLen (bn_v b)) i ==
            index #uint8 #len (nat_to_intseq_le #U8 len (bn_v b)) i) =
-    index_nat_to_intseq_le #U8 #SEC (bnLen * 8) (bn_v b) i;
+    index_nat_to_intseq_le #U8 #SEC tmpLen (bn_v b) i;
     index_nat_to_intseq_le #U8 #SEC len (bn_v b) i in
 
   Classical.forall_intro aux;
